Cleaning. dispatching in different files.

spark2cmproofs.v
@@ -1,263 +1,34 @@
 
-Require Import Utf8.
-Require Import function_utils.
-Require Import LibHypsNaming.
-Require Import Errors.
-Require Import spark2Cminor.
-Require Import Cminor.
+Require Import
+  ZArith Utf8 function_utils LibHypsNaming Errors spark2Cminor Cminor
+  symboltable semantics semantics_properties Sorted Relations
+  compcert.lib.Integers compcert_utils more_stdlib.
+
 Require Ctypes.
-Require Import symboltable.
-Require Import semantics.
-Require Import semantics_properties.
-Require Import Sorted.
-Require Import Relations.
-Require Import Integers.
+Import Symbol_Table_Module Memory.
 
-Lemma wordsize_ok : wordsize = Integers.Int.wordsize.
-Proof.
-  reflexivity.
-Qed.
-
-Lemma modulus_ok: modulus = Integers.Int.modulus.
-Proof.
-  reflexivity.
-Qed.
-
-Lemma half_modulus_ok: half_modulus = Integers.Int.half_modulus.
-Proof.
-  reflexivity.
-Qed.
-
-Lemma max_unsigned_ok: max_unsigned = Integers.Int.max_unsigned.
-Proof.
-  reflexivity.
-Qed.
-
-Lemma max_signed_ok: max_signed = Integers.Int.max_signed.
-Proof.
-  reflexivity.
-Qed.
-
-Lemma min_signed_ok: min_signed = Integers.Int.min_signed.
-Proof.
-  reflexivity.
-Qed.
-
-(* All element of a sorted list are smaller or equal to the first
-   element. If the ordering is reflexive. *)
-Lemma increasing_order_In A :
-  forall (ord:A -> A -> Prop) (stk:list A) (hd:A),
-    StronglySorted ord (hd::stk) ->
-    Forall (fun elt => elt = hd \/ ord hd elt) (hd::stk).
-Proof.
-  !intros.
-  !inversion H.
-  constructor 2.
-  - left;reflexivity.
-  - apply Forall_forall.
-    !intros.
-    right.
-    rewrite Forall_forall in H3.
-    auto.
-Qed.
-
-
-Import Symbol_Table_Module.
 Open Scope error_monad_scope.
-
 Open Scope Z_scope.
 
-(* Auxiliary lemmas, should go in Compcert? *)
-Lemma repr_inj:
-  forall v1 v2,
-    Integers.Int.min_signed <= v1 <= Integers.Int.max_signed ->
-    Integers.Int.min_signed <= v2 <= Integers.Int.max_signed ->
-    Integers.Int.repr v1 = Integers.Int.repr v2 ->
-    v1 = v2.
-Proof.
-  intros v1 v2 hinbound1 hinboun2.
-  !intros.
-  assert (h: Integers.Int.signed(Integers.Int.repr v1)
-             = Integers.Int.signed(Integers.Int.repr v2)).
-  { rewrite heq. reflexivity. }
-  rewrite Integers.Int.signed_repr in h;auto.
-  rewrite Integers.Int.signed_repr in h;auto.
-Qed.
-
-Lemma repr_inj_neq:
-  forall v1 v2,
-    Integers.Int.min_signed <= v1 <= Integers.Int.max_signed ->
-    Integers.Int.min_signed <= v2 <= Integers.Int.max_signed ->
-    v1 <> v2 -> 
-    Integers.Int.repr v1 <> Integers.Int.repr v2.
-Proof.
-  intros v1 v2 hinbound1 hinboun2 hneq.
-  intro abs.
-  apply repr_inj in abs;auto.
-Qed.
-
-(* These should be part of std lib maybe.  *)
-
-Lemma Zneq_bool_false: forall x y : Z, x = y -> Zneq_bool x y = false.
-Proof.
-  !intros.
-  subst.
-  unfold Zneq_bool.
-  rewrite Fcore_Zaux.Zcompare_Eq;auto.
-Qed.
-  
-Lemma Zneq_bool_true: forall x y : Z, x <> y -> Zneq_bool x y = true.
-Proof.
-  intros x y hneq.
-  apply Z.lt_gt_cases in hneq.
-  !destruct hneq.
-  - unfold Zneq_bool.
-    rewrite Fcore_Zaux.Zcompare_Lt;auto.
-  - unfold Zneq_bool.
-    rewrite Fcore_Zaux.Zcompare_Gt;auto.
-Qed.
-
-(* TODO: replace this y the real typing function *)
-Definition type_of_name (stbl:symboltable) (nme:name): res type :=
-  match nme with
-    | E_Identifier astnum id => fetch_var_type id stbl
-    | E_Indexed_Component astnum x0 x1 => Error (msg "type_of_name: arrays not treated yet")
-    | E_Selected_Component astnum x0 x1 => Error (msg "transl_basetype: records not treated yet")
-  end.
-
-
-
-
-(** Hypothesis renaming stuff *)
-Ltac rename_hyp1 h th :=
+(** Hypothesis renaming stuff from other files *)
+Ltac rename_hyp_prev h th :=
   match th with
-    | ?min <= ?x and ?x < ?max => fresh "h_" x "_bounded_" min "_" max 
-    | ?min <= ?x and ?x < ?max => fresh "h_" x "_bounded_"
-    | ?min <= ?x and ?x < ?max => fresh "h_bounded"
-
-    | fetch_var_type _ _ = Error _ => fresh "heq_fetch_var_type_ERR"
-    | fetch_var_type _ _ = _ => fresh "heq_fetch_var_type"
-    | fetch_exp_type _ _ = Error _ => fresh "heq_fetch_exp_type_ERR"
-    | compute_chnk _ ?name = OK ?chk => fresh "heq_compute_chnk_" name "_" chk
-    | compute_chnk _ ?name = ?chk => fresh "heq_compute_chnk_" name "_" chk
-    | compute_chnk _ ?name = _ => fresh "heq_compute_chnk_" name
-    | compute_chnk _ _ = _ => fresh "heq_compute_chnk"
-    | symboltable.fetch_exp_type _ _ = _ => fresh "heq_fetch_exp_type"
-    | symboltable.fetch_exp_type _ _ = Error _ => fresh "heq_fetch_exp_type_ERR"
-    | fetch_exp_type _ _ = _ => fresh "heq_fetch_exp_type" (* symboltable.fetch_exp_type *)
-    | eval_expr _ _ _ (Run_Time_Error _) => fresh "h_eval_expr_RE"
-    | eval_expr _ _ _ (Normal ?v) => fresh "h_eval_expr_" v
-    | eval_expr _ _ _ ?v => fresh "h_eval_expr_" v
-    | eval_expr _ _ _ _ => fresh "h_eval_expr"
-    | eval_name _ _ _ (Run_Time_Error _) => fresh "h_eval_name_RE"
-    | eval_name _ _ _ (Normal ?v) => fresh "h_eval_name_" v
-    | eval_name _ _ _ ?v => fresh "h_eval_name_" v
-    | eval_name _ _ _ _ => fresh "h_eval_name"
-    | do_overflow_check _ (Run_Time_Error _) => fresh "h_overf_check_RE"
-    | do_overflow_check _ _ => fresh "h_overf_check"
-    | do_range_check _ _ _ (Run_Time_Error _) => fresh "h_do_range_check_RE"
-    | do_range_check _ _ _ _ => fresh "h_do_range_check"
-    | do_run_time_check_on_binop _ _ _ (Run_Time_Error _) => fresh "h_do_rtc_binop_RTE"
-    | do_run_time_check_on_binop _ _ _ _ => fresh "h_do_rtc_binop"
-    | Ctypes.access_mode ?x = _ => fresh "h_access_mode_" x
-    | Ctypes.access_mode _ = _ => fresh "h_access_mode"
-    | Cminor.exec_stmt _ _ _ _ _ _ _ _ _ None  => fresh "h_exec_stmt_None"
-    | Cminor.exec_stmt _ _ _ _ _ _ _ _ _ _  => fresh "h_exec_stmt"
-    | Cminor.eval_constant _ _ _ = (Some _)  => fresh "h_eval_constant"
-    | Cminor.eval_constant _ _ _ = None  => fresh "h_eval_constant_None"
-    | eval_literal _ (Run_Time_Error _)  => fresh "h_eval_literal_RE"
-    | eval_literal _ _  => fresh "h_eval_literal"
-    | eval_stmt _ _ _ (Run_Time_Error _) => fresh "h_eval_stmt_RE"
-    | eval_stmt _ _ _ _ => fresh "h_eval_stmt"
-    | transl_stmt _ _ _ = Error _ => fresh "heq_transl_stmt_ERR"
-    | transl_stmt _ _ _ = _ => fresh "heq_transl_stmt"
-    | transl_name _ _ _ = Error _ => fresh "heq_transl_name_ERR"
-    | transl_name _ _ _ = _ => fresh "heq_transl_name"
-    | Cminor.eval_expr _ _ _ _ ?x _ => fresh "h_CM_eval_expr_" x
-    | Cminor.eval_expr _ _ _ _ _ _ => fresh "h_CM_eval_expr"
-    | transl_value _ Error _ => fresh "heq_transl_value_RE"
-    | transl_value _ _ => fresh "heq_transl_value"
-    | transl_variable _ _ _ _ = Error _ => fresh "heq_transl_variable_RE"
-    | transl_variable _ _ _ _ = _ => fresh "heq_transl_variable"
-    | fetch_exp_type _ _ = Some _ => fresh "heq_fetch_exp_type"
-    | fetch_exp_type _ _ = None => fresh "heq_fetch_exp_type_none"
-    | transl_type _ _ = Error _ => fresh "heq_transl_type_RE"
-    | transl_type _ _ = _ => fresh "heq_transl_type"
-    | transl_basetype _ _ = Error _ => fresh "heq_transl_basetype_RE"
-    | transl_basetype _ _ = _ => fresh "heq_transl_basetype"
-    | build_loads ?n ?z = _ => fresh "heq_build_loads_" n "_" z
-    | build_loads _ _ = _ => fresh "heq_build_loads"
-    | make_load _ _ = Error _ => fresh "heq_make_load_RE"
-    | make_load _ _ = _ => fresh "heq_make_load"
-    | STACK.fetchG _ _ = Some _ => fresh "heq_SfetchG"
-    | STACK.fetchG _ _ = None => fresh "heq_SfetchG_none"
-    | storeUpdate _ _ _ _ (Run_Time_Error _) => fresh "h_storeupdate_RTE"
-    | storeUpdate _ _ _ _ _ => fresh "h_storeupdate"
-    | do_run_time_check_on_binop _ _ _ (Run_Time_Error _) =>  fresh "h_do_rtc_binop_RE"
-    | do_run_time_check_on_binop _ _ _ _ =>  fresh "h_do_rtc_binop"
-    | do_run_time_check_on_unop _ _ (Run_Time_Error _) =>  fresh "h_do_rtc_unop_RE"
-    | do_run_time_check_on_unop _ _ _ =>  fresh "h_do_rtc_unop"
-    | reduce_type _ _ _ = Error _ => fresh "heq_reduce_type_RE"
-    | reduce_type _ _ _ = _  => fresh "heq_reduce_type"
-    | concrete_type_of_value _ = Error _ => fresh "concrete_type_of_value_RE"
-    | concrete_type_of_value _ = _ => fresh "concrete_type_of_value"
-    | in_bound _ _ _ => fresh "h_inbound"
-    | do_division_check _ _ (Run_Time_Error _) => fresh "h_do_division_check_RTE"
-    | do_division_check _ _ _ => fresh "h_do_division_check"
-
-    | CompilEnv.fetchG ?id ?CE = _ => fresh "heq_CEfetchG_" id "_" CE
-    | CompilEnv.fetchG ?id _ = _ => fresh "heq_CEfetchG_" id
-    | CompilEnv.fetchG _ _ = Some _ => fresh "heq_CEfetchG"
-    | CompilEnv.fetchG _ _ = None => fresh "heq_CMfetchG_none"
-
-    | CompilEnv.fetch ?id ?CE = _ => fresh "heq_CEfetch_" id "_" CE
-    | CompilEnv.fetch ?id _ = _ => fresh "heq_CEfetch_" id
-    | CompilEnv.fetch _ _ = Some _ => fresh "heq_CEfetch"
-    | CompilEnv.fetch _ _ = None => fresh "heq_CMfetch_none"
-
-    | CompilEnv.frameG ?id ?CE = _ => fresh "heq_CEframeG_" id "_" CE
-    | CompilEnv.frameG ?id _ = _ => fresh "heq_CEframeG_" id
-    | CompilEnv.frameG _ _ = Some _ => fresh "heq_CEframeG"
-    | CompilEnv.frameG _ _ = None => fresh "heq_CMframeG_none"
-
-    | CompilEnv.level_of_top ?ce = None => fresh "heq_lvloftop_none_" ce
-    | CompilEnv.level_of_top ?ce = None => fresh "heq_lvloftop_none"
-    | CompilEnv.level_of_top ?ce = Some ?s => fresh "heq_lvloftop_" ce "_" s
-    | CompilEnv.level_of_top ?ce = ?s => fresh "heq_lvloftop_" ce "_" s
-    | CompilEnv.level_of_top ?ce = _ => fresh "heq_lvloftop_" ce
-    | CompilEnv.level_of_top _ = Some ?s => fresh "heq_lvloftop_" s
-    | CompilEnv.level_of_top _ = _ => fresh "heq_lvloftop"
-
-    | Memory.Mem.store ?chk ?m ?blk ?n ?v = None => fresh "heq_store_" v "_none"
-    | Memory.Mem.store ?chk ?m ?blk ?n ?v = OK ?m2 => fresh "heq_store_" v "_" m2
-    | Memory.Mem.store ?chk ?m ?blk ?n ?v = ?m2 => fresh "heq_store_" v "_" m2
-    | Memory.Mem.store ?chk ?m ?blk ?n ?v = ?m2 => fresh "heq_store_" v
-    | Memory.Mem.store ?chk ?m ?blk ?n ?v = ?m2 => fresh "heq_store"
-
-    | Memory.Mem.storev ?chk ?m ?vaddr ?v = None => fresh "heq_storev_" v "_none"
-    | Memory.Mem.storev ?chk ?m ?vaddr ?v = OK ?m2 => fresh "heq_storev_" v "_" m2
-    | Memory.Mem.storev ?chk ?m ?vaddr ?v = ?m2 => fresh "heq_storev_" v "_" m2
-    | Memory.Mem.storev ?chk ?m ?vaddr ?v = ?m2 => fresh "heq_storev_" v
-    | Memory.Mem.storev ?chk ?m ?vaddr ?v = ?m2 => fresh "heq_storev"
-
-
-    | transl_expr ?stbl ?CE ?e = Error => fresh "heq_tr_expr_none"
-    | transl_expr ?stbl ?CE ?e = OK ?r => fresh "heq_tr_expr_" e
-    | transl_expr ?stbl ?CE ?e = ?r => fresh "heq_tr_expr"
-
-
-    (* TODO: remove when we remove type_of_name by the real one. *)
-    | type_of_name _ _ = Error _ => fresh "heq_type_of_name_ERR"
-    | type_of_name _ _ = _ => fresh "heq_type_of_name"
+    | _ => (semantics_properties.rename_hyp1 h th)
+    | _ => (spark2Cminor.rename_hyp1 h th)
+    | _ => (compcert_utils.rename_hyp1 h th)
   end.
 
+Ltac rename_hyp ::= rename_hyp_prev.
 
+
+(* Removal of uninformative equalities *)
 Ltac remove_refl :=
   repeat
     match goal with
       | H: ?e = ?e |- _ => clear H
     end.
 
+(* + exploiting equalities. *)
 Ltac eq_same_clear :=
   repeat progress
     (repeat remove_refl;
@@ -268,7 +39,65 @@ Ltac eq_same_clear :=
               | H: ?A <> ?A |- _ => elim H;reflexivity
             end).
 
+
+(* basic notions coincides between compcert and spark *)
+Lemma wordsize_ok : wordsize = Integers.Int.wordsize.
+Proof. reflexivity. Qed.
+
+Lemma modulus_ok: modulus = Integers.Int.modulus.
+Proof. reflexivity. Qed.
+
+Lemma half_modulus_ok: half_modulus = Integers.Int.half_modulus.
+Proof. reflexivity. Qed.
+
+Lemma max_unsigned_ok: max_unsigned = Integers.Int.max_unsigned.
+Proof. reflexivity. Qed.
+
+Lemma max_signed_ok: max_signed = Integers.Int.max_signed.
+Proof. reflexivity. Qed.
+
+Lemma min_signed_ok: min_signed = Integers.Int.min_signed.
+Proof. reflexivity. Qed.
+
+(* TODO: replace this y the real typing function *)
+Definition type_of_name (stbl:symboltable) (nme:name): res type :=
+  match nme with
+    | E_Identifier astnum id => fetch_var_type id stbl
+    | E_Indexed_Component astnum x0 x1 => Error (msg "type_of_name: arrays not treated yet")
+    | E_Selected_Component astnum x0 x1 => Error (msg "transl_basetype: records not treated yet")
+  end.
+
+
+(** Hypothesis renaming stuff *)
+Ltac rename_hyp1 h th :=
+  match th with
+    (* TODO: remove when we remove type_of_name by the real one. *)
+    | type_of_name _ _ = Error _ => fresh "heq_type_of_name_ERR"
+    | type_of_name _ _ = _ => fresh "heq_type_of_name"
+    | _ => (rename_hyp_prev h th)
+  end.
+
 Ltac rename_hyp ::= rename_hyp1.
+
+
+Lemma transl_value_det: forall v tv1 tv2,
+    transl_value v tv1 -> transl_value v tv2 -> tv1 = tv2.
+Proof.
+  !intros.
+  inversion heq_transl_value0; inversion heq_transl_value;subst;auto;inversion H1;auto.
+Qed.
+
+
+Lemma transl_value_tot: forall v,
+        (forall y:nat,(exists b, v = Bool b \/ exists n, v = Int n))
+          -> exists tv, transl_value v tv.
+Proof.
+  !intros.
+  decomp (H 0%nat);subst.
+  - destruct x;eexists;econstructor.
+  - eexists;econstructor.
+Qed.
+
 
 Lemma transl_literal_ok1 :
   forall g (l:literal) v,
@@ -334,37 +163,39 @@ Ltac inv_if_intop op h :=
    end.
 
 (* Transform hypothesis of the form do_range_check into disequalities. *)
+(* shortening the name to shorten the tactic below *)
+Notation rtc_binop := do_run_time_check_on_binop (only parsing).
 Ltac inv_rtc :=
   repeat
     progress
     (try match goal with
-           | H: do_run_time_check_on_binop ?op Undefined _ (Normal _) |- _ => now inversion H
-           | H: do_run_time_check_on_binop ?op _ Undefined (Normal _) |- _ => now inversion H
-           | H: do_run_time_check_on_binop ?op _ (ArrayV _) (Normal _) |- _ => now inv_if_intop op H
-           | H: do_run_time_check_on_binop ?op (ArrayV _) _ (Normal _) |- _ => now inv_if_intop op H
-           | H: do_run_time_check_on_binop ?op _ (RecordV _) (Normal _) |- _ => now inv_if_intop op H
-           | H: do_run_time_check_on_binop ?op (RecordV _) _ (Normal _) |- _ => now inv_if_intop op H
-           | H: do_run_time_check_on_binop ?op _ (Bool _) (Normal _) |- _ => inv_if_intop op H
-           | H: Math.binary_operation ?op _ (Bool _) = (Some _) |- _ => inv_if_intop op H
-           | H: do_run_time_check_on_binop ?op (Bool _) _ (Normal _) |- _ => inv_if_intop op H
-           | H: Math.binary_operation ?op (Bool _) _ = (Some _) |- _ => inv_if_intop op H
-           | H: do_overflow_check _ (Normal (Int _)) |- _ => !invclear H
-           | H: do_range_check _ _ _ (Normal (Int _)) |- _ => !invclear H
-           | H: in_bound _ _ true |- _ => !invclear H
-           | H:(_ >=? _) && (_ >=? _) = true |- _ =>
-             rewrite andb_true_iff in H;
-           try rewrite Z.geb_le in H;
-           try rewrite Z.geb_le in H;
-           let h1 := fresh "h_le"in
-           let h2 := fresh "h_le"in
-           destruct H as [h1 h2 ]
-           | H:(_ <=? _) && (_ <=? _) = true |- _ =>
-             rewrite andb_true_iff in H;
-           try rewrite Z.leb_le in H;
-           try rewrite Z.leb_le in H;
-           let h1 := fresh "h_le"in
-           let h2 := fresh "h_le"in
-           destruct H as [h1 h2 ]
+         | H: rtc_binop ?op Undefined _ (Normal _) |- _ => now inversion H
+         | H: rtc_binop ?op _ Undefined (Normal _) |- _ => now inversion H
+         | H: rtc_binop ?op _ (ArrayV _) (Normal _) |- _ => now inv_if_intop op H
+         | H: rtc_binop ?op (ArrayV _) _ (Normal _) |- _ => now inv_if_intop op H
+         | H: rtc_binop ?op _ (RecordV _) (Normal _) |- _ => now inv_if_intop op H
+         | H: rtc_binop ?op (RecordV _) _ (Normal _) |- _ => now inv_if_intop op H
+         | H: rtc_binop ?op _ (Bool _) (Normal _) |- _ => inv_if_intop op H
+         | H: Math.binary_operation ?op _ (Bool _) = (Some _) |- _ => inv_if_intop op H
+         | H: rtc_binop ?op (Bool _) _ (Normal _) |- _ => inv_if_intop op H
+         | H: Math.binary_operation ?op (Bool _) _ = (Some _) |- _ => inv_if_intop op H
+         | H: do_overflow_check _ (Normal (Int _)) |- _ => !invclear H
+         | H: do_range_check _ _ _ (Normal (Int _)) |- _ => !invclear H
+         | H: in_bound _ _ true |- _ => !invclear H
+         | H:(_ >=? _) && (_ >=? _) = true |- _ =>
+           rewrite andb_true_iff in H;
+             try rewrite Z.geb_le in H;
+             try rewrite Z.geb_le in H;
+             let h1 := fresh "h_le"in
+             let h2 := fresh "h_le"in
+             destruct H as [h1 h2 ]
+         | H:(_ <=? _) && (_ <=? _) = true |- _ =>
+           rewrite andb_true_iff in H;
+             try rewrite Z.leb_le in H;
+             try rewrite Z.leb_le in H;
+             let h1 := fresh "h_le" in
+             let h2 := fresh "h_le" in
+             destruct H as [h1 h2 ]
          end; auto 2).
 
 
@@ -378,9 +209,9 @@ Lemma not_ok: forall v1 v0 x,
 Proof.
   !intros.
   !destruct v1;try discriminate;simpl in *;eq_same_clear.
-  !destruct n;simpl in *
-  ; inversion heq_transl_value
-  ; constructor.
+  !destruct n;simpl in *;
+  inversion heq_transl_value;
+  constructor.
 Qed.
 
 
@@ -476,7 +307,10 @@ Proof.
   !destruct v1;try discriminate; !destruct v2;try discriminate;simpl in *;eq_same_clear.
   !destruct (Z.eq_dec n n0).
   - subst.
-    rewrite Zneq_bool_false;auto.
+    replace (Zneq_bool n0 n0) with false. all:swap 1 2. {
+      symmetry.
+      apply Zneq_bool_false_iff.
+      reflexivity. }
     unfold Values.Val.cmp.
     inversion heq_transl_value0;subst;simpl.
     inversion heq_transl_value;subst;simpl.
@@ -787,8 +621,7 @@ Proof.
       destruct h_divoverf as [h_divoverf1 h_divoverf2].
       exfalso.
       assert (v1_is_min_int: v1 = Integers.Int.min_signed).
-      { 
-        rewrite Integers.Int.eq_signed in h_divoverf1.
+      { rewrite Integers.Int.eq_signed in h_divoverf1.
         unfold Coqlib.zeq in h_divoverf1;auto.
         rewrite !Integers.Int.signed_repr in h_divoverf1;try (split;omega).
         destruct (Z.eq_dec v1 Integers.Int.min_signed);try discriminate.
@@ -822,24 +655,6 @@ Proof.
     + split;auto.
 Qed.
 
-Lemma transl_value_det: forall v tv1 tv2,
-    transl_value v tv1 -> transl_value v tv2 -> tv1 = tv2.
-Proof.
-!intros.
-  inversion heq_transl_value0; inversion heq_transl_value;subst;auto;inversion H1;auto.
-                                                                                    Qed.
-Tactic Notation "decomp" constr(h) :=
-  !! (fun x => decompose [and ex or] x; try clear x) h.
-
-Lemma transl_value_tot: forall v,
-        (forall y:nat,(exists b, v = Bool b \/ exists n, v = Int n))
-          -> exists tv, transl_value v tv.
-Proof.
-  !intros.
-  decomp (H 0%nat);subst.
-  - destruct x;eexists;econstructor.
-  - eexists;econstructor.
-Qed.
 
 Lemma binary_operator_ok:
   forall op (n n1 n2 : Values.val) (v v1 v2 : value),
@@ -895,10 +710,23 @@ Proof.
 Qed.
 
 
+(** * Memory invariant and bisimilarity *)
 
 
-(** [safe_stack s] means that every value in s is correct wrt to
-    overflows.
+Lemma eval_literal_overf :
+  forall (l:literal) n, 
+    eval_literal l (Normal (Int n)) ->
+    do_overflow_check n (Normal (Int n)).
+Proof.
+  !intros.
+  !inversion h_eval_literal.
+  !inversion h_overf_check.
+  assumption.
+Qed.
+
+
+(** [safe_stack s] means that every value in the spark stack [s] is
+    correct wrt to overflows.
     TODO: extend with other values than Int: floats, arrays, records. *)
 Definition safe_stack s :=
   forall id n,
@@ -914,18 +742,6 @@ Ltac rename_hyp2' h th :=
   end.
 
 Ltac rename_hyp ::= rename_hyp2'.
-
-Lemma eval_literal_overf :
-  forall (l:literal) n, 
-    eval_literal l (Normal (Int n)) ->
-    do_overflow_check n (Normal (Int n)).
-Proof.
-  !intros.
-  !inversion h_eval_literal.
-  !inversion h_overf_check.
-  assumption.
-Qed.
-
 
 Lemma eval_name_overf : forall s st nme n,
                           safe_stack s
@@ -960,11 +776,13 @@ Proof.
     + inversion h_overf_check;subst;auto.
     + inversion h_overf_check;subst;auto.
     + rewrite binopexp_ok in *.
-      functional inversion heq;subst;try match goal with H: ?A <> ?A |- _ => elim H;auto end.
+      functional inversion heq;subst
+      ;try match goal with H: ?A <> ?A |- _ => elim H;auto end.
   - !invclear h_do_rtc_unop.
     + inversion h_overf_check;subst;auto.
     + rewrite unopexp_ok in *.
-      !functional inversion heq;subst;try match goal with H: ?A <> ?A |- _ => elim H;auto end.
+      !functional inversion heq;subst
+      ;try match goal with H: ?A <> ?A |- _ => elim H;auto end.
       !invclear heq2.
       apply IHh_eval_expr;auto.
 Qed.
@@ -1029,30 +847,54 @@ Definition stack_separate st CE sp locenv g m :=
      \/ Int.unsigned δ₂ + Memdata.size_chunk chnk₂ <= Int.unsigned δ₁
      \/ Int.unsigned δ₁ + Memdata.size_chunk chnk₁ <= Int.unsigned δ₂).
 
+Definition increasing_order: localframe -> Prop :=
+  StronglySorted (fun x y => snd x > snd y).
+
+Definition increasing_order_fr (f:CompilEnv.frame) :=
+  increasing_order(CompilEnv.store_of f).
+
+Definition increasing_orderG (stk: CompilEnv.stack): Prop :=
+  StronglySorted (fun x y => (CompilEnv.level_of x > CompilEnv.level_of y)%nat) stk.
+
 (* See CminorgenProof.v@205. *)
-(* We will need more than that probably. But for now let us use
-   a simple notion of matching: the value of a variable is equal to
-   the value of its translation. Its translation is currently (an
-   expression of the form ELoad((Eload(Eload ...(Eload(0)))) + n)). We
-   could define a specialization of eval_expr for this kind of
-   expression but at some point the form of the expression will
-   complexify (some variables may stay temporary instead of going in
-   the stack, etc).
 
-   We also put well-typing constraints on the stack wrt symbol
-   table. *)
+(** The Memory bisimilarity/invariant property states that
 
+ - Spark stack [s] is ok wrt overflows
+ - Compilation environment [CE] contains exactly variables of spark
+   stack [s]
+ - All variable of [CE] are non overlapping (spark property)
+ - The structure of the chaines stack in Cminor is maintained:
+ -- Load (Load...(Load 0)) yields to some frame f and a null offset
+    ([localstack_aligned])
+ -- and no variable overlap with it ([no_null_offset]).
+ - the value of a variable is equal to the value of its translation.
+   Its translation is currently (an expression of the form
+   ELoad((Eload(Eload ...(Eload(0)))) + n)).
+ - spark variables and there translated address yield the same
+   (translated) value. i.e. the two memories commute. *)
 Record match_env (st:symboltable) (s: STACK.stack)
        (CE:compilenv) (sp:Values.val) (locenv: Cminor.env)
-       (g:genv)(m:Memory.Mem.mem): Prop :=
+       (g:genv)(m:Mem.mem): Prop :=
   mk_match_env {
       me_stack_match: stack_match st s CE sp locenv g m;
       me_stack_complete: stack_complete st s CE;
       me_stack_separate: stack_separate st CE sp locenv g m;
       me_stack_localstack_aligned: stack_localstack_aligned locenv g m;
       me_stack_no_null_offset: stack_no_null_offset st CE;
-      me_overflow: safe_stack s
+      me_overflow: safe_stack s (* Put this somewhere else, concerns only s *)
     }.
+
+(** The compilation environment has some intrinsic properties:
+ - Frame are numbered in increasing order in the global store
+ - In each frame variables are numbered in increasing order
+ - variable addresses do not overflow. *)
+Record invariant_compile CE :=
+  { increasing_lvls: increasing_orderG CE ;
+    increasing_ids: Forall (λ otherfrm, increasing_order_fr otherfrm) CE ;
+    no_overflow: (∀ id δ, CompilEnv.fetchG id CE = Some δ → 0 <= δ ∧ δ < Int.modulus) }.
+
+Hint Resolve increasing_lvls increasing_ids no_overflow.
 
 
 (** Hypothesis renaming stuff *)
@@ -1102,8 +944,9 @@ Ltac rename_hyp4 h th :=
   end.
 Ltac rename_hyp ::= rename_hyp4.
 
-(* Property of the translation: Since chain variables have always zero
-   offset, the offset of a variable in CE is the CMinor one. *)
+(** Property of the translation: Since chain variables have always zero
+   offset, the offset of a variable in CE is the same as its offset in
+   CMinor memory. *)
 Lemma eval_build_loads_offset: forall g stkptr locenv m δ_lvl δ_id b ofs,
     stack_localstack_aligned locenv g m ->
     Cminor.eval_expr g stkptr locenv m (build_loads δ_lvl δ_id) (Values.Vptr b ofs) ->
@@ -1125,8 +968,8 @@ Proof.
 Qed.
 
 
-(* Property of the translation: Since chain variables have always zero
-   offset, the offset of a variable in CE is more than 3. *)
+(** Property of the translation: Since chain variables have always
+    zero offset, the offset of a variable in CE must be more than 3. *)
 Lemma eval_build_loads_offset_non_null_var: forall stbl CE g stkptr locenv m nme a bld_lds b ofs,
     stack_no_null_offset stbl CE ->
     stack_localstack_aligned locenv g m ->
@@ -1262,14 +1105,43 @@ Ltac rename_hyp5 th :=
 
 Ltac rename_hyp ::= rename_hyp5.
 
-      
+Scheme Equality for binary_operator.
+Scheme Equality for unary_operator.
+Scheme Equality for literal.
+  
+Ltac finish_eqdec := try subst;try (left;reflexivity);(try now right;intro abs;inversion abs;contradiction).
 
+Lemma expression_dec: forall e1 e2:expression, ({e1=e2} + {e1<>e2})
+with name_dec: forall n1 n2:name, ({n1=n2} + {n1<>n2}).
+Proof.
+  { !intros.
+    case e1;case e2;intros;try now((left+right)).
+    - destruct (Nat.eq_dec a0 a);finish_eqdec.
+      destruct (literal_eq_dec l0 l);finish_eqdec.
+    - destruct (Nat.eq_dec a0 a);finish_eqdec.
+      destruct (name_dec n0 n);finish_eqdec.
+    - destruct (Nat.eq_dec a0 a);finish_eqdec.
+      destruct (binary_operator_eq_dec b0 b);finish_eqdec.
+      destruct (expression_dec e3 e);finish_eqdec.
+      destruct (expression_dec e4 e0);finish_eqdec.
+    - destruct (Nat.eq_dec a0 a);finish_eqdec.
+      destruct (unary_operator_eq_dec u0 u);finish_eqdec.
+      destruct (expression_dec e0 e);finish_eqdec. }
+  { !intros.
+    case n1;case n2;intros;finish_eqdec.
+    - destruct (Nat.eq_dec a0 a);finish_eqdec.
+      destruct (Nat.eq_dec i0 i);finish_eqdec.
+    - destruct (Nat.eq_dec a0 a);finish_eqdec.
+      destruct (name_dec n0 n);finish_eqdec.
+      destruct (expression_dec e0 e);finish_eqdec.
+    - destruct (Nat.eq_dec a0 a);finish_eqdec.
+      destruct (name_dec n0 n);finish_eqdec.
+      destruct (Nat.eq_dec i0 i);finish_eqdec. }
+Defined.
 
-Axiom expression_dec: forall e1 e2:expression, ({e1=e2} + {e1<>e2}).
-Axiom name_dec: forall e1 e2:name, {e1=e2} + {e1<>e2}. 
 
 Import STACK.
-
+(* Is this true? *)
 Axiom det_eval_expr: forall g stkptr locenv m e v v',
                        Cminor.eval_expr g stkptr locenv m e v
                        -> Cminor.eval_expr g stkptr locenv m e v'
@@ -1355,14 +1227,6 @@ Proof.
   apply IHl₂;auto.
 Qed.
 
-
-Lemma neq_sym : forall A, forall x y : A , x<>y  -> y<>x.
-Proof.
-  intros A x y H.
-  intro abs.
-  subst.
-  apply H;reflexivity.
-Qed.
 
 Lemma build_loads__inj :
   forall i₁ i₂,
@@ -1530,80 +1394,6 @@ Qed.
 
 
 
-Require Import FMapList.
-Require Import OrderedType.
-
-(*
-Inductive increasing_order : localframe -> Prop :=
-  IncO : increasing_order []
-| IncNext: forall lf id δ,
-    increasing_order lf ->
-    (forall otherid y', CompilEnv.fetches otherid lf = Some y' -> δ < y') ->
-    increasing_order ((id,δ)::lf).
-*)
-(*
-Module localframeORD <: OrderedType.
-  Definition t := (idnum * CompilEnv.V)%type.
-  
-  Definition eq := @eq t.
-  Definition lt := (fun x y:t => snd x < snd y).
-
-  Definition eq_refl := @eq_refl t.
-  Definition eq_sym := @eq_sym t.
-  Definition eq_trans := @eq_trans t.
-  Opaque eq_refl eq_sym eq_trans.
-
-  Lemma lt_not_eq : forall m1 m2 : t, lt m1 m2 -> ~ eq m1 m2.
-  Proof.
-    !intros.
-    unfold eq , lt in *.
-    intro abs.
-    subst.
-    destruct (Z.lt_irrefl _ H).
-  Qed.
-  Lemma lt_irrefl: bool.
-    exact true.
-  Qed.
-  Lemma lt_antisym :symmetric _ lt.
-  Proof.
-    admit.
-  Qed.
-      
-  Lemma lt_trans:transitive _ lt.
-  Proof.
-    unfold transitive.
-    !intros.
-    unfold lt in *.
-    eapply Zlt_trans;eauto.
-  Qed.
-
-
-
-End localframeORD.
-MSetList.Make().
-*)
-Definition increasing_order: localframe -> Prop := StronglySorted (fun x y => snd x > snd y).
-
-Definition increasing_order_fr (f:CompilEnv.frame) :=
-  increasing_order(CompilEnv.store_of f).
-
-
-(* FIXME: find another name *)
-(* levels of each substack are ordered *)
-(*
-Inductive increasing_orderG : CompilEnv.stack -> Prop :=
-  IncOG : increasing_orderG []
-| IncNextG: forall stk frm,
-    increasing_orderG stk ->
-    increasing_order_fr frm ->
-    (List.Forall
-       (fun otherfrm =>
-          (CompilEnv.level_of otherfrm < CompilEnv.level_of frm)%nat)
-       stk) ->
-    increasing_orderG (frm::stk).
-*)
-Definition increasing_orderG (stk: CompilEnv.stack): Prop :=
-  StronglySorted (fun x y => (CompilEnv.level_of x > CompilEnv.level_of y)%nat) stk.
 
 
 
@@ -1624,72 +1414,69 @@ Ltac rename_hyp_incro h th :=
   end.
 Ltac rename_hyp ::= rename_hyp_incro.
 
-Section mapping.
-  
-(*   Variable (stbl: symboltable) (CE:compilenv) (locenv : env) (g : genv) (stkptr:Values.val). *)
-  
-  Lemma increase_order_level_of_top_ge:
-    forall CE id s s0 s3,
-      increasing_orderG CE ->
-      CompilEnv.frameG id CE = Some (s, s0) ->
-      CompilEnv.level_of_top CE = Some s3 -> 
-      (s3 >= s)%nat.
-  Proof.
-    !intros.
-    unfold increasing_orderG in *.
-    !destruct CE;!intros.
-    - simpl in *;try discriminate.
-    - specialize (increasing_order_In _ _ _ _ h_incr_orderG_CE).
-      !intro.
-      rewrite Forall_forall in h_forall.
-      apply Nat.lt_eq_cases.
-      unfold CompilEnv.level_of in *.
-      apply frameG_In in heq_CEframeG_id_CE.
-      specialize (h_forall _ heq_CEframeG_id_CE).
-      !destruct f.
-      unfold CompilEnv.level_of_top in heq_lvloftop_CE_s3.
-      simpl in *.
-      !invclear heq_lvloftop_CE_s3.
-      !destruct h_forall;auto.
-      inject heq;auto.
-  Qed.
+
+Lemma increase_order_level_of_top_ge:
+  forall CE id s s0 s3,
+    increasing_orderG CE ->
+    CompilEnv.frameG id CE = Some (s, s0) ->
+    CompilEnv.level_of_top CE = Some s3 -> 
+    (s3 >= s)%nat.
+Proof.
+  !intros.
+  unfold increasing_orderG in *.
+  !destruct CE;!intros.
+  - simpl in *;try discriminate.
+  - specialize (increasing_order_In _ _ _ _ h_incr_orderG_CE).
+    !intro.
+    rewrite Forall_forall in h_forall.
+    apply Nat.lt_eq_cases.
+    unfold CompilEnv.level_of in *.
+    apply frameG_In in heq_CEframeG_id_CE.
+    specialize (h_forall _ heq_CEframeG_id_CE).
+    !destruct f.
+    unfold CompilEnv.level_of_top in heq_lvloftop_CE_s3.
+    simpl in *.
+    !invclear heq_lvloftop_CE_s3.
+    !destruct h_forall;auto.
+    inject heq;auto.
+Qed.
 
 
-  Lemma CEfetches_inj : forall id₁ id₂ (lf:localframe) δ₁ δ₂,
-      increasing_order lf ->
-      CompilEnv.fetches id₁ lf = Some δ₁ ->
-      CompilEnv.fetches id₂ lf = Some δ₂ ->
-      id₁ ≠ id₂ ->
-      δ₁ ≠ δ₂.
-  Proof.
-    intros until lf.
-    !induction lf;simpl in *;!intros.
-    - discriminate.
-    - destruct a.
-      destruct (Nat.eq_dec id₁ i);subst.
-      + rewrite Nat.eqb_refl in heq0.
-        !invclear heq0.
-        assert (h:id₂ ≠ i) by auto.
-        rewrite <- (Nat.eqb_neq id₂ i) in h.
-        rewrite h in heq.
+Lemma CEfetches_inj : forall id₁ id₂ (lf:localframe) δ₁ δ₂,
+    increasing_order lf ->
+    CompilEnv.fetches id₁ lf = Some δ₁ ->
+    CompilEnv.fetches id₂ lf = Some δ₂ ->
+    id₁ ≠ id₂ ->
+    δ₁ ≠ δ₂.
+Proof.
+  intros until lf.
+  !induction lf;simpl in *;!intros.
+  - discriminate.
+  - destruct a.
+    destruct (Nat.eq_dec id₁ i);subst.
+    + rewrite Nat.eqb_refl in heq0.
+      !invclear heq0.
+      assert (h:id₂ ≠ i) by auto.
+      rewrite <- (Nat.eqb_neq id₂ i) in h.
+      rewrite h in heq.
+      inversion h_incr_order;subst;simpl in *.
+      assert (δ₁ > δ₂). {
+        rewrite Forall_forall in H2.
+        eapply (H2 (id₂,δ₂));eauto.
+        apply fetches_In.
+        assumption. }
+      symmetry.
+      apply Z.lt_neq.
+      apply Z.gt_lt_iff.
+      assumption.
+    + destruct (Nat.eq_dec id₂ i).
+      * subst.
+        rewrite Nat.eqb_refl in heq.
+        !invclear heq.
+        assert (h:id₁ ≠ i) by auto.
+        rewrite <- (Nat.eqb_neq id₁ i) in h.
+        rewrite h in heq0.
         inversion h_incr_order;subst;simpl in *.
-        assert (δ₁ > δ₂). {
-          rewrite Forall_forall in H2.
-          eapply (H2 (id₂,δ₂));eauto.
-          apply fetches_In.
-          assumption. }
-        apply neq_sym.
-        apply Z.lt_neq.
-        apply Z.gt_lt_iff.
-        assumption.
-      + destruct (Nat.eq_dec id₂ i).
-        * subst.
-          rewrite Nat.eqb_refl in heq.
-          !invclear heq.
-          assert (h:id₁ ≠ i) by auto.
-          rewrite <- (Nat.eqb_neq id₁ i) in h.
-          rewrite h in heq0.
-          inversion h_incr_order;subst;simpl in *.
         assert (δ₂ > δ₁). {
           rewrite Forall_forall in H2.
           eapply (H2 (id₁,δ₁));eauto.
@@ -1698,1015 +1485,779 @@ Section mapping.
         apply Z.lt_neq.
         apply Z.gt_lt_iff.
         assumption.
-        * rewrite <- (Nat.eqb_neq id₁ i) in n.
-          rewrite <- (Nat.eqb_neq id₂ i) in n0.
-          rewrite n,n0 in *.
-          apply IHlf;auto.
-          inversion h_incr_order.
-          assumption.
-  Qed.
+      * rewrite <- (Nat.eqb_neq id₁ i) in n.
+        rewrite <- (Nat.eqb_neq id₂ i) in n0.
+        rewrite n,n0 in *.
+        apply IHlf;auto.
+        inversion h_incr_order.
+        assumption.
+Qed.
 
 
-  Lemma CEfetch_inj : forall id₁ id₂ (a:CompilEnv.frame) δ₁ δ₂,
-      increasing_order_fr a ->
-      CompilEnv.fetch id₁ a = Some δ₁ ->
-      CompilEnv.fetch id₂ a = Some δ₂ ->
+Lemma CEfetch_inj : forall id₁ id₂ (a:CompilEnv.frame) δ₁ δ₂,
+    increasing_order_fr a ->
+    CompilEnv.fetch id₁ a = Some δ₁ ->
+    CompilEnv.fetch id₂ a = Some δ₂ ->
+    id₁ ≠ id₂ ->
+    δ₁ ≠ δ₂.
+Proof.
+  intros until a.
+  unfold CompilEnv.fetch.
+  !destruct a;simpl.
+  unfold increasing_order_fr.
+  simpl.
+  apply CEfetches_inj.
+Qed.
+
+Lemma CEfetchG_inj : forall CE id₁ id₂,
+    increasing_orderG CE ->
+    List.Forall (fun otherfrm => increasing_order_fr otherfrm) CE ->
+    forall  δ₁ δ₂ k₁ k₂ frm₁ frm₂,
+      CompilEnv.fetchG id₁ CE = Some δ₁ ->
+      CompilEnv.fetchG id₂ CE = Some δ₂ ->
+      CompilEnv.frameG id₁ CE = Some (k₁, frm₁) ->
+      CompilEnv.frameG id₂ CE = Some (k₂, frm₂) ->
       id₁ ≠ id₂ ->
-      δ₁ ≠ δ₂.
-  Proof.
-    intros until a.
-    unfold CompilEnv.fetch.
-    !destruct a;simpl.
-    unfold increasing_order_fr.
-    simpl.
-    apply CEfetches_inj.
-  Qed.
-
-Set Printing Width 75.
-  Lemma CEfetchG_inj : forall CE id₁ id₂,
-      increasing_orderG CE ->
-      List.Forall (fun otherfrm => increasing_order_fr otherfrm) CE ->
-      forall  δ₁ δ₂ k₁ k₂ frm₁ frm₂,
-        CompilEnv.fetchG id₁ CE = Some δ₁ ->
-        CompilEnv.fetchG id₂ CE = Some δ₂ ->
-        CompilEnv.frameG id₁ CE = Some (k₁, frm₁) ->
-        CompilEnv.frameG id₂ CE = Some (k₂, frm₂) ->
-        id₁ ≠ id₂ ->
-        (k₁ <> k₂ \/ δ₁ <> δ₂).
-  Proof.
-    intros until 0.
-    !intro.
-    !induction h_incr_orderG_CE;!intros;simpl in *;try discriminate.
-    rewrite Forall_forall in h_forall_l, h_forall.
-    unfold CompilEnv.level_of in *.
-    destruct (CompilEnv.fetch id₁ a) eqn:heq_fetch_id₁;
-      destruct (CompilEnv.fetch id₂ a) eqn:heq_fetch_id₂;
-      eq_same_clear;subst;simpl in *;try discriminate.
-    - right.
-      eapply CEfetch_inj;eauto.
-    - left.
-      apply neq_sym.
-      apply Nat.lt_neq.
-      apply CEfetch_reside_false in heq_fetch_id₂.
-      apply CEfetch_reside_true in heq_fetch_id₁.
-      rewrite heq_fetch_id₂,heq_fetch_id₁ in *;simpl in *.
-      !invclear heq_CEframeG_id₁;simpl in *.
-      specialize (h_forall_l (lvl_id₂, fr_id₂)).
-      simpl in *.
-      apply h_forall_l.
-      eapply frameG_In;eauto.
-    - left.
-      apply Nat.lt_neq.
-      apply CEfetch_reside_true in heq_fetch_id₂.
-      apply CEfetch_reside_false in heq_fetch_id₁.
-      rewrite heq_fetch_id₂,heq_fetch_id₁ in *;simpl in *.
-      !invclear heq_CEframeG_id₂;simpl in *.
-      specialize (h_forall_l (lvl_id₁, fr_id₁)).
-      simpl in *.
-      apply h_forall_l.
-      eapply frameG_In;eauto.
-    - apply CEfetch_reside_false in heq_fetch_id₁.
-      apply CEfetch_reside_false in heq_fetch_id₂.
-      rewrite heq_fetch_id₁,heq_fetch_id₂ in *.
-      eapply IHh_incr_orderG_CE ;eauto.
-      rewrite Forall_forall.
-      intros x H.
-      apply h_forall;auto.
-  Qed.
+      (k₁ <> k₂ \/ δ₁ <> δ₂).
+Proof.
+  intros until 0.
+  !intro.
+  !induction h_incr_orderG_CE;!intros;simpl in *;try discriminate.
+  rewrite Forall_forall in h_forall_l, h_forall.
+  unfold CompilEnv.level_of in *.
+  destruct (CompilEnv.fetch id₁ a) eqn:heq_fetch_id₁;
+    destruct (CompilEnv.fetch id₂ a) eqn:heq_fetch_id₂;
+    eq_same_clear;subst;simpl in *;try discriminate.
+  - right.
+    eapply CEfetch_inj;eauto.
+  - left.
+    symmetry.
+    apply Nat.lt_neq.
+    apply CEfetch_reside_false in heq_fetch_id₂.
+    apply CEfetch_reside_true in heq_fetch_id₁.
+    rewrite heq_fetch_id₂,heq_fetch_id₁ in *;simpl in *.
+    !invclear heq_CEframeG_id₁;simpl in *.
+    specialize (h_forall_l (lvl_id₂, fr_id₂)).
+    simpl in *.
+    apply h_forall_l.
+    eapply frameG_In;eauto.
+  - left.
+    apply Nat.lt_neq.
+    apply CEfetch_reside_true in heq_fetch_id₂.
+    apply CEfetch_reside_false in heq_fetch_id₁.
+    rewrite heq_fetch_id₂,heq_fetch_id₁ in *;simpl in *.
+    !invclear heq_CEframeG_id₂;simpl in *.
+    specialize (h_forall_l (lvl_id₁, fr_id₁)).
+    simpl in *.
+    apply h_forall_l.
+    eapply frameG_In;eauto.
+  - apply CEfetch_reside_false in heq_fetch_id₁.
+    apply CEfetch_reside_false in heq_fetch_id₂.
+    rewrite heq_fetch_id₁,heq_fetch_id₂ in *.
+    eapply IHh_incr_orderG_CE ;eauto.
+    rewrite Forall_forall.
+    intros x H.
+    apply h_forall;auto.
+Qed.
 
 
-  Lemma minus_same_eq : forall s3 s s1,
+Lemma minus_same_eq : forall s3 s s1,
     s ≤ s3 ->
     s1 ≤ s3 ->
     (s3 - s1)%nat = (s3 - s)%nat ->
     s = s1.
-  Proof.
-    induction s3;intros.
-    - inversion H0;inversion H;auto.
-    - inversion H;inversion H0;subst.
-      + reflexivity.
-      + rewrite minus_diag in H1.
-        apply Nat.sub_0_le in H1.
-        assert (s3 < s3)%nat. {
-          eapply lt_le_trans with s1;auto. }
-        destruct (lt_irrefl s3);auto.
-      + rewrite minus_diag in H1.
-        symmetry in H1.
-        apply Nat.sub_0_le in H1.
-        assert (s3 < s3)%nat. {
-          eapply lt_le_trans with s;auto. }
-        destruct (lt_irrefl s3);auto.
-      + eapply IHs3;eauto.
-        setoid_rewrite <- minus_Sn_m in H1;auto.
-  Qed.
+Proof.
+  induction s3;intros.
+  - inversion H0;inversion H;auto.
+  - inversion H;inversion H0;subst.
+    + reflexivity.
+    + rewrite minus_diag in H1.
+      apply Nat.sub_0_le in H1.
+      assert (s3 < s3)%nat. {
+        eapply lt_le_trans with s1;auto. }
+      destruct (lt_irrefl s3);auto.
+    + rewrite minus_diag in H1.
+      symmetry in H1.
+      apply Nat.sub_0_le in H1.
+      assert (s3 < s3)%nat. {
+        eapply lt_le_trans with s;auto. }
+      destruct (lt_irrefl s3);auto.
+    + eapply IHs3;eauto.
+      setoid_rewrite <- minus_Sn_m in H1;auto.
+Qed.
 
-  Lemma minus_same_neq : forall s3 s s1,
+Lemma minus_same_neq : forall s3 s s1,
     s ≤ s3 ->
     s1 ≤ s3 ->
     s <> s1 ->
     (s3 - s1)%nat <> (s3 - s)%nat.
-  Proof.
-    !intros.
-    intro abs.
-    apply minus_same_eq in abs;auto.
-  Qed.
+Proof.
+  !intros.
+  intro abs.
+  apply minus_same_eq in abs;auto.
+Qed.
 
 
-  Lemma transl_variable_inj :
-    forall CE stbl a₁ a₂ id₁ id₂ k₁ k₂ δ₁ δ₂,
-      (* Frame are numbered with different (increasing) numers *)
-      increasing_orderG CE ->
-      (* In each frame, stacks are also numbered with (increasing) numbers *)
-      List.Forall (fun otherfrm => increasing_order_fr otherfrm) CE ->
-      (forall id δ, CompilEnv.fetchG id CE = Some δ -> 0 <= δ ∧ δ < Integers.Int.modulus) ->
-      (* translating the variabe to a Cminor load address *)
-      transl_variable stbl CE a₁ id₁ = OK (build_loads k₁ δ₁) ->
-      (* translating the variabe to a Cminor load address *)
-      transl_variable stbl CE a₂ id₂ = OK   (build_loads k₂ δ₂) ->
-      id₁ <> id₂ ->
-      (k₁ <> k₂ \/ δ₁<> δ₂).
-  Proof.
-    !intros.
-    match goal with
-    | H: appcontext [(0 <= _) ∧ (_ < Integers.Int.modulus)] |- _ => rename H into h_bound_CE
-    end.
-    unfold transl_variable in *.
-    destruct (CompilEnv.fetchG id₁ CE) eqn:h₁;simpl in *;try discriminate.
-    destruct (CompilEnv.fetchG id₂ CE) eqn:h₂;simpl in *;try discriminate.
-    destruct (CompilEnv.frameG id₁ CE) eqn:h₁';simpl in *;try discriminate.
-    destruct (CompilEnv.frameG id₂ CE) eqn:h₂';simpl in *;try discriminate.
-    destruct f.
-    destruct f0.
-    assert (hh:=CEfetchG_inj _ _ _ h_incr_orderG_CE h_forall_CE _ _ _ _ _ _  h₁ h₂ h₁' h₂' hneq).
-    destruct (CompilEnv.level_of_top CE) eqn:hlvlofCE.
-    - (* remember here refrain inversion to bizarrely unfold too much. *)
-      remember (build_loads (s3 - s1) t0) as fooo.
-      remember (build_loads (s3 - s) t) as fooo'.
-      inversion heq_transl_variable as [heqfoo].
-      inversion heq_transl_variable0 as [heqfoo'].
-      clear heq_transl_variable heq_transl_variable0.
-      subst.
-      apply build_loads_inj in heqfoo.
-      apply build_loads_inj in heqfoo'.
-      !destruct heqfoo.
-      !destruct heqfoo'.
-      subst.
-      !destruct hh.
-      + left.
-        eapply minus_same_neq;eauto.
-        eapply increase_order_level_of_top_ge;eauto.
-        eapply increase_order_level_of_top_ge;eauto.
-      + repeat rewrite Integers.Int.Z_mod_modulus_eq in *.
-        rewrite Coqlib.Zmod_small in *;eauto.
-        subst.
-        right.
-        intro abs.
-        subst.
-        apply hneq0;reflexivity.
-    - discriminate.
-  Qed.
-
-(*
-  (* We need something more precise, probably this: *)
-  Lemma foo2 :
-    forall stbl chnk₁ chnk₂ a₁ a₂ id₁ id₂ k₁ k₂ δ₁ δ₂,
-      (* Frame are numbered with different (increasing) numers *)
-      increasing_orderG CE ->
-      (* In each frame, stacks are also numbered with (increasing) numbers *)
-      List.Forall (fun otherfrm => increasing_order_fr otherfrm) CE ->
-      (forall id δ, CompilEnv.fetchG id CE = Some δ
-                    -> 0 <= δ ∧ δ < Integers.Int.modulus) ->
-      (* translating the variabe to a Cminor load address *)
-      transl_variable stbl CE a₁ id₁ = OK (build_loads k₁ δ₁) ->
-      (* translating the variabe to a Cminor load address *)
-      transl_variable stbl CE a₂ id₂ = OK (build_loads k₂ δ₂) ->
-      compute_chnk_id stbl id₁ = OK chnk₁ ->
-      compute_chnk_id stbl id₂ = OK chnk₂ ->
-      id₁ <> id₂ ->
-      (k₁ <> k₂
-       \/ δ₂ + Memdata.size_chunk chnk₂ <= δ₁
-       \/ δ₁ + Memdata.size_chunk chnk₁ <= δ₂).
-  Proof.
-  Admitted.
-
-
-    (* We need something more precise, probably this: *)
-  Lemma foo2' :
-    forall stbl chnk₁ a₁  id₁ k₁ δ₁,
-      (* Frame are numbered with different (increasing) numers *)
-      increasing_orderG CE ->
-      (* In each frame, stacks are also numbered with (increasing) numbers *)
-      List.Forall (fun otherfrm => increasing_order_fr otherfrm) CE ->
-      (forall id δ, CompilEnv.fetchG id CE = Some δ
-                    -> 0 <= δ ∧ δ < Integers.Int.modulus) ->
-      (* translating the variabe to a Cminor load address *)
-      transl_variable stbl CE a₁ id₁ = OK (build_loads k₁ δ₁) ->
-      compute_chnk_id stbl id₁ = OK chnk₁ ->
-      forall chnk₂ a₂ id₂ k₂ δ₂,
-        (* translating the variabe to a Cminor load address *)
-        transl_variable stbl CE a₂ id₂ = OK (build_loads k₂ δ₂) ->
-        compute_chnk_id stbl id₂ = OK chnk₂ ->
-        id₁ <> id₂ ->
-        (k₁ <> k₂
-         \/ δ₂ + Memdata.size_chunk chnk₂ <= δ₁
-         \/ δ₁ + Memdata.size_chunk chnk₁ <= δ₂).
-  Proof.
-  Admitted.*)
-(*
-  (* TODO: simplify this proof. *)
-  Lemma cmtype_chk : forall tpnme t tt chk,
-      transl_type stbl tpnme = OK t -> 
-      Ctypes.opttyp_of_type t = Some tt ->
-      Ctypes.access_mode t = Ctypes.By_value chk ->
-      chk = AST.chunk_of_type tt.
-  Proof.
-    intros.
-    functional inversion H;subst;simpl in *;eq_same_clear;simpl in *.
-    - inversion H1;auto.
-    - inversion H1;auto.
-    - destruct t;simpl in *;try discriminate;eq_same_clear;
-      try
-        now
-        repeat
-        match goal with
-        | h:function_utils.transl_typenum _ _ = OK _ |- _ =>
-          try functional inversion h;eq_same_clear;subst; try clear h
-        | h:function_utils.transl_basetype _ _  =
-            OK _ |- _ => try functional inversion h;eq_same_clear;subst; try clear h
-        | h:Ctypes.By_value _ = Ctypes.By_value _ |- _ => !invclear h;auto
-        end.
-
-      + destruct i;simpl in *;
-        try
-          now
-          repeat
-          match goal with
-          | h:function_utils.transl_typenum _ _ = OK _ |- _ =>
-            try functional inversion h;eq_same_clear;subst; try clear h
-          | h:function_utils.transl_basetype _ _  =
-              OK _ |- _ => try functional inversion h;eq_same_clear;subst; try clear h
-          | h:Ctypes.By_value _ = Ctypes.By_value _ |- _ => !invclear h;auto
-          end;
-        destruct s;simpl in *; try rewrite <- transl_typenum_ok in *;
-        repeat match goal with
-               | h:function_utils.transl_typenum _ _ = OK _ |- _ =>
-                 try functional inversion h;eq_same_clear;subst; try clear h
-               | h:function_utils.transl_basetype _ _  =
-                   OK _ |- _ => try functional inversion h;eq_same_clear;subst; try clear h
-               | h:Ctypes.By_value _ = Ctypes.By_value _ |- _ => !invclear h;auto
-               end.
-      + try rewrite <- transl_typenum_ok in *;
-        repeat match goal with
-               | h:function_utils.transl_typenum _ _ = OK _ |- _ =>
-                 try functional inversion h;eq_same_clear;subst; try clear h
-               | h:function_utils.transl_basetype _ _  =
-                   OK _ |- _ => try functional inversion h;eq_same_clear;subst; try clear h
-               | h:Ctypes.By_value _ = Ctypes.By_value _ |- _ => !invclear h;auto
-               end.
-    - destruct t;simpl in *;try discriminate;eq_same_clear;
-      try
-        now
-        repeat
-        match goal with
-        | h:function_utils.transl_typenum _ _ = OK _ |- _ =>
-          try functional inversion h;eq_same_clear;subst; try clear h
-        | h:function_utils.transl_basetype _ _  =
-            OK _ |- _ => try functional inversion h;eq_same_clear;subst; try clear h
-        | h:Ctypes.By_value _ = Ctypes.By_value _ |- _ => !invclear h;auto
-        end.
-
-      + destruct i;simpl in *;
-        try
-          now
-          repeat
-          match goal with
-          | h:function_utils.transl_typenum _ _ = OK _ |- _ =>
-            try functional inversion h;eq_same_clear;subst; try clear h
-          | h:function_utils.transl_basetype _ _  =
-              OK _ |- _ => try functional inversion h;eq_same_clear;subst; try clear h
-          | h:Ctypes.By_value _ = Ctypes.By_value _ |- _ => !invclear h;auto
-          end;
-        destruct s;simpl in *; try rewrite <- transl_typenum_ok in *;
-        repeat match goal with
-               | h:function_utils.transl_typenum _ _ = OK _ |- _ =>
-                 try functional inversion h;eq_same_clear;subst; try clear h
-               | h:function_utils.transl_basetype _ _  =
-                   OK _ |- _ => try functional inversion h;eq_same_clear;subst; try clear h
-               | h:Ctypes.By_value _ = Ctypes.By_value _ |- _ => !invclear h;auto
-               end.
-      + try rewrite <- transl_typenum_ok in *;
-        repeat match goal with
-               | h:function_utils.transl_typenum _ _ = OK _ |- _ =>
-                 try functional inversion h;eq_same_clear;subst; try clear h
-               | h:function_utils.transl_basetype _ _  =
-                   OK _ |- _ => try functional inversion h;eq_same_clear;subst; try clear h
-               | h:Ctypes.By_value _ = Ctypes.By_value _ |- _ => !invclear h;auto
-               end.
-    - destruct t;simpl in *;try discriminate;eq_same_clear;
-      try
-        now
-        repeat
-        match goal with
-        | h:function_utils.transl_typenum _ _ = OK _ |- _ =>
-          try functional inversion h;eq_same_clear;subst; try clear h
-        | h:function_utils.transl_basetype _ _  =
-            OK _ |- _ => try functional inversion h;eq_same_clear;subst; try clear h
-        | h:Ctypes.By_value _ = Ctypes.By_value _ |- _ => !invclear h;auto
-        end.
-
-      + destruct i;simpl in *;
-        try
-          now
-          repeat
-          match goal with
-          | h:function_utils.transl_typenum _ _ = OK _ |- _ =>
-            try functional inversion h;eq_same_clear;subst; try clear h
-          | h:function_utils.transl_basetype _ _  =
-              OK _ |- _ => try functional inversion h;eq_same_clear;subst; try clear h
-          | h:Ctypes.By_value _ = Ctypes.By_value _ |- _ => !invclear h;auto
-          end;
-        destruct s;simpl in *; try rewrite <- transl_typenum_ok in *;
-        repeat match goal with
-               | h:function_utils.transl_typenum _ _ = OK _ |- _ =>
-                 try functional inversion h;eq_same_clear;subst; try clear h
-               | h:function_utils.transl_basetype _ _  =
-                   OK _ |- _ => try functional inversion h;eq_same_clear;subst; try clear h
-               | h:Ctypes.By_value _ = Ctypes.By_value _ |- _ => !invclear h;auto
-               end.
-      + try rewrite <- transl_typenum_ok in *;
-        repeat match goal with
-               | h:function_utils.transl_typenum _ _ = OK _ |- _ =>
-                 try functional inversion h;eq_same_clear;subst; try clear h
-               | h:function_utils.transl_basetype _ _  =
-                   OK _ |- _ => try functional inversion h;eq_same_clear;subst; try clear h
-               | h:Ctypes.By_value _ = Ctypes.By_value _ |- _ => !invclear h;auto
-               end.
-    - destruct t;simpl in *;try discriminate;eq_same_clear;
-      try
-        now
-        repeat
-        match goal with
-        | h:function_utils.transl_typenum _ _ = OK _ |- _ =>
-          try functional inversion h;eq_same_clear;subst; try clear h
-        | h:function_utils.transl_basetype _ _  =
-            OK _ |- _ => try functional inversion h;eq_same_clear;subst; try clear h
-        | h:Ctypes.By_value _ = Ctypes.By_value _ |- _ => !invclear h;auto
-        end.
-
-      + destruct i;simpl in *;
-        try
-          now
-          repeat
-          match goal with
-          | h:function_utils.transl_typenum _ _ = OK _ |- _ =>
-            try functional inversion h;eq_same_clear;subst; try clear h
-          | h:function_utils.transl_basetype _ _  =
-              OK _ |- _ => try functional inversion h;eq_same_clear;subst; try clear h
-          | h:Ctypes.By_value _ = Ctypes.By_value _ |- _ => !invclear h;auto
-          end;
-        destruct s;simpl in *; try rewrite <- transl_typenum_ok in *;
-        repeat match goal with
-               | h:function_utils.transl_typenum _ _ = OK _ |- _ =>
-                 try functional inversion h;eq_same_clear;subst; try clear h
-               | h:function_utils.transl_basetype _ _  =
-                   OK _ |- _ => try functional inversion h;eq_same_clear;subst; try clear h
-               | h:Ctypes.By_value _ = Ctypes.By_value _ |- _ => !invclear h;auto
-               end.
-      + try rewrite <- transl_typenum_ok in *;
-        repeat match goal with
-               | h:function_utils.transl_typenum _ _ = OK _ |- _ =>
-                 try functional inversion h;eq_same_clear;subst; try clear h
-               | h:function_utils.transl_basetype _ _  =
-                   OK _ |- _ => try functional inversion h;eq_same_clear;subst; try clear h
-               | h:Ctypes.By_value _ = Ctypes.By_value _ |- _ => !invclear h;auto
-               end.
-  Qed.
-*)
-  Lemma transl_variable_astnum:
-    forall stbl CE astnum id' addrof_nme,
-      transl_variable stbl CE astnum id' = OK addrof_nme
-      -> forall a,transl_variable stbl CE a id' = transl_variable stbl CE astnum id'.
-  Proof.
-    !intros.
-    unfold transl_variable.
-    !functional inversion heq_transl_variable.
-    rewrite  heq_CEfetchG_id'_CE, heq_CEframeG_id'_CE, heq_lvloftop_CE_m'.
-    reflexivity.
-  Qed.
-
-
-
-  Lemma compute_chk_32 :
-    forall stbl t,
-      compute_chnk_of_type stbl t = OK AST.Mint32
-      -> transl_type stbl t = OK (Ctypes.Tint Ctypes.I32 Ctypes.Signed Ctypes.noattr).
-  Proof.
-    !intros.
-    functional inversion heq;subst;simpl.
-    - functional inversion H;simpl.
-      reflexivity.
-    - functional inversion H;simpl.
-      reflexivity.
-  Qed.
-
-  Set Printing Width 80.
-
-
-
-  Notation " x =: y" := (x = OK y) (at level 90).
-  Notation " x =! y" := (x = Error y) (at level 120).
-
-  Ltac simplify_do :=
-    repeat progress
-           (match goal with
-            | H: context [do _ <- ?e ; _] , H': ?e = _ |- _ =>
-              rewrite H' in H;simpl in H
-            | H': ?e = _ |- context [do _ <- ?e ; _]  =>
-              rewrite H';simpl
-            end).
-
-
-  (* Well-formedness of the chained stack: store never modify the
-     address of a variable. Reason: since variable addresses are
-     expressions of the form ((Load(Load(...(Load 0))))+δ) with δ >= 4
-     and that stores never touch the addresses 0, variables addresses
-     never change. *)
-  Lemma wf_chain_load'2:forall g locenv stkptr chk m m' b ofs e_t_v
-                             vaddr,
-      Memory.Mem.storev chk m (Values.Vptr b ofs) e_t_v = Some m'
-      -> (stack_localstack_aligned locenv g m)
-      -> (4 <= (Int.unsigned ofs))(*forall n, Integers.Int.repr n = ofs -> 4 <= n*)
-      -> forall lvl,
-          let load_id := build_loads_ lvl in
-          Cminor.eval_expr g stkptr locenv m' load_id vaddr
-          -> Cminor.eval_expr g stkptr locenv m load_id vaddr.
-  Proof.
-    !intros.
-    rename H1 into h_ofs_non_zero.
-    simpl in *.
-    subst load_id.
-    generalize dependent vaddr.
-    induction lvl;!intros;simpl in *.
-    - !inversion h_CM_eval_expr;econstructor;eauto.
-    - !invclear h_CM_eval_expr.
-      assert (h_CM_eval_expr_on_m:Cminor.eval_expr g stkptr locenv m (build_loads_ lvl) vaddr0). { eapply IHlvl; eauto. }
-      econstructor.
-      + eassumption.
-      + destruct vaddr0;simpl in *;try discriminate.
-        rewrite <- heq.
-        symmetry.
-        eapply Memory.Mem.load_store_other;eauto.
-        right.
-        left.
-        simpl.
-        transitivity 4.
-        * !destruct (h_aligned_g_m _ _ _ h_CM_eval_expr_on_m).
-          !invclear heq.
-          !invclear heq0.
-          vm_compute.
-          intro abs;discriminate.
-        * apply h_ofs_non_zero.
-  Qed.
-
-  (* Well-formedness of the chained stack: store never modify the
-     address of a variable. Reason: since variable addresses are
-     expressions of the form ((Load(Load(...(Load 0))))+δ) with δ >= 4
-     and that stores never touch the addresses 0, variables addresses
-     never change. *)
-  Lemma wf_chain_load'3:forall g locenv stkptr chk m m' b ofs e_t_v
-                             vaddr,
-      Memory.Mem.storev chk m (Values.Vptr b ofs) e_t_v = Some m'
-      -> stack_localstack_aligned locenv g m'
-      -> (4 <= (Int.unsigned ofs))(*forall n, Integers.Int.repr n = ofs -> 4 <= n*)
-      -> forall lvl,
-          let load_id := build_loads_ lvl in
-          Cminor.eval_expr g stkptr locenv m load_id vaddr
-          -> Cminor.eval_expr g stkptr locenv m' load_id vaddr.
-  Proof.
-    !intros.
-    rename H1 into h_ofs_non_zero.
-    simpl in *.
-    subst load_id.
-    generalize dependent vaddr.
-    induction lvl;!intros;simpl in *.
-    - !inversion h_CM_eval_expr;econstructor;eauto.
-    - !invclear h_CM_eval_expr.
-      assert (h_CM_eval_expr_on_m':Cminor.eval_expr g stkptr locenv m' (build_loads_ lvl) vaddr0). { eapply IHlvl; eauto. }
-      econstructor.
-      + eassumption.
-      + destruct vaddr0;simpl in *;try discriminate.
-        rewrite <- heq.
-        eapply Memory.Mem.load_store_other;eauto.
-        right.
-        left.
-        simpl.
-        transitivity 4.
-        * !destruct (h_aligned_g_m' _ _ _ h_CM_eval_expr_on_m').
-          !invclear heq.
-          !invclear heq0.
-          vm_compute.
-          intro abs;discriminate.
-        * apply h_ofs_non_zero.
-  Qed.
-
-
-  Lemma wf_chain_load'':forall g locenv stkptr chk m m' b ofs e_t_v
-                             vaddr,
-      Memory.Mem.storev chk m (Values.Vptr b ofs) e_t_v = Some m'
-      -> (stack_localstack_aligned locenv g m)
-      -> (stack_localstack_aligned locenv g m')
-      -> (4 <= (Int.unsigned ofs))(*forall n, Integers.Int.repr n = ofs -> 4 <= n*)
-      -> forall lvl,
-          let load_id := build_loads_ lvl in
-          Cminor.eval_expr g stkptr locenv m' load_id vaddr
-          <-> Cminor.eval_expr g stkptr locenv m load_id vaddr.
-  Proof.
-    intros g locenv stkptr chk m m' b ofs e_t_v vaddr H H0 H1 H2 lvl load_id.
-    split;intro .
-    - eapply wf_chain_load'2 ;eauto.
-    - eapply wf_chain_load'3 ;eauto.
-  Qed.
-
-  (* Well-formedness of the chained stack: store never modify the
-     address of a variable. Reason: since variable addresses are
-     expressions of the form ((Load(Load(...(Load 0))))+δ) with δ >= 4
-     and that stores never touch the addresses 0, variables addresses
-     never change. *)
-  Lemma wf_chain_load':forall g locenv stkptr chk m m' b ofs e_t_v
-                             vaddr,
-      Memory.Mem.storev chk m (Values.Vptr b ofs) e_t_v = Some m'
-      -> (stack_localstack_aligned locenv g m')
-      -> (4 <= (Int.unsigned ofs))(*forall n, Integers.Int.repr n = ofs -> 4 <= n*)
-      -> forall lvl δ_lvl,
-          let load_id := build_loads lvl δ_lvl in
-          Cminor.eval_expr g stkptr locenv m load_id vaddr
-          -> Cminor.eval_expr g stkptr locenv m' load_id vaddr.
-  Proof.
-    !intros.
-    rename H1 into h_ofs_non_zero.
-    simpl in *.
-    unfold build_loads in *.
-    !invclear h_CM_eval_expr_load_id.
-    econstructor;eauto.
-    Focus 2.
-    { inversion h_CM_eval_expr;econstructor;eauto. }
-    Unfocus.
-    eapply wf_chain_load'3;eauto.
-  Qed.
-
-  (* Well-formedness of the chained stack: store never modify the
-     address of a variable. Reason: since variable addresses are
-     expressions of the form ((Load(Load(...(Load 0))))+δ) with δ >= 4
-     and that stores never touch the addresses 0, variables addresses
-     never change. *)
-  Lemma wf_chain_load'_2:forall g locenv stkptr chk m m' b ofs e_t_v
-                             vaddr,
-      Memory.Mem.storev chk m (Values.Vptr b ofs) e_t_v = Some m'
-      -> (stack_localstack_aligned locenv g m)
-      -> (4 <= (Int.unsigned ofs))(*forall n, Integers.Int.repr n = ofs -> 4 <= n*)
-      -> forall lvl δ_lvl,
-          let load_id := build_loads lvl δ_lvl in
-          Cminor.eval_expr g stkptr locenv m' load_id vaddr
-          -> Cminor.eval_expr g stkptr locenv m load_id vaddr.
-  Proof.
-    !intros.
-    rename H1 into h_ofs_non_zero.
-    simpl in *.
-    unfold build_loads in *.
-    !invclear h_CM_eval_expr_load_id.
-    econstructor;eauto.
-    Focus 2.
-    { inversion h_CM_eval_expr;econstructor;eauto. }
-    Unfocus.
-    eapply wf_chain_load'2;eauto.
-  Qed.
-
-  (* Well-formedness of the chained stack: store never modify the
-     address of a variable. Reason: since variable addresses are
-     expressions of the form ((Load(Load(...(Load 0))))+δ) with δ >= 4
-     and that stores never touch the addresses 0, variables addresses
-     never change. *)
-  Lemma wf_chain_load_var:forall stbl CE g locenv stkptr astnum chk m m' b ofs e_t_v
-                             id load_id vaddr,
-      Memory.Mem.storev chk m (Values.Vptr b ofs) e_t_v = Some m'
-      -> (stack_localstack_aligned locenv g m')
-      -> (4 <= (Int.unsigned ofs))(*forall n, Integers.Int.repr n = ofs -> 4 <= n*)
-      -> transl_variable stbl CE astnum id =: load_id
-      -> Cminor.eval_expr g stkptr locenv m load_id vaddr
-      -> Cminor.eval_expr g stkptr locenv m' load_id vaddr.
-  Proof.
-    !intros.
-    rename H1 into h_ofs_non_zero.
-    simpl in *.
-    !functional inversion heq_transl_variable;subst;clear heq_transl_variable.
-    rename m'0 into max_lvl.
-    set (δ_lvl:=(max_lvl - lvl_id)%nat) in *.
-    eapply wf_chain_load';eauto.
-  Qed.
-
-  (* Well-formedness of the chained stack: store never modify the
-     address of a variable. Reason: since variable addresses are
-     expressions of the form ((Load(Load(...(Load 0))))+δ) with δ >= 4
-     and that stores never touch the addresses 0, variables addresses
-     never change. *)
-  Lemma wf_chain_load_var':forall stbl CE g locenv stkptr astnum chk m m' b ofs e_t_v
-                             id load_id vaddr,
-      Memory.Mem.storev chk m (Values.Vptr b ofs) e_t_v = Some m'
-      -> (stack_localstack_aligned locenv g m)
-      -> (4 <= (Int.unsigned ofs))(*forall n, Integers.Int.repr n = ofs -> 4 <= n*)
-      -> transl_variable stbl CE astnum id =: load_id
-      -> Cminor.eval_expr g stkptr locenv m' load_id vaddr
-      -> Cminor.eval_expr g stkptr locenv m load_id vaddr.
-  Proof.
-    !intros.
-    rename H1 into h_ofs_non_zero.
-    simpl in *.
-    !functional inversion heq_transl_variable;subst;clear heq_transl_variable.
-    rename m'0 into max_lvl.
-    set (δ_lvl:=(max_lvl - lvl_id)%nat) in *.
-    eapply wf_chain_load'_2;eauto.
-  Qed.
-
-
-
-
-  Set Printing Width 100.
-
-
-
-  (* INVARIANT OF STORE/STOREV: if we do not touch on addresses zero
-     of blocks, chaining variables all poitn to zero ofsets. *)
-  Lemma wf_chain_load_aligned:forall g locenv chk m m' b ofs e_t_v,
-      Memory.Mem.storev chk m (Values.Vptr b ofs) e_t_v = Some m'
-      -> (4 <= (Int.unsigned ofs))
-      -> stack_localstack_aligned locenv g m
-      -> stack_localstack_aligned locenv g m'.
-  Proof.
-    unfold stack_localstack_aligned at 2.
-    !intros.
-    revert g locenv chk m m' b ofs e_t_v heq_storev_e_t_v H0 h_aligned_g_m b0 v h_CM_eval_expr.
-    destruct δ_lvl;simpl;!intros.
-    - rename h_aligned_g_m0 into h_aligned_m.
-      rename h_CM_eval_expr0 into h_CM_eval_expr.
-      edestruct (h_aligned_m b0 O v).
-      + simpl.
-        constructor.
-        !inversion h_CM_eval_expr.
-        assumption.
-      + eauto.
-    - rename h_aligned_g_m0 into h_aligned_m.
-      rename h_CM_eval_expr0 into h_CM_eval_expr.
-      !inversion h_CM_eval_expr.
-      generalize h_CM_eval_expr0.
-      !intro.
-      eapply wf_chain_load'2 in h_CM_eval_expr2;eauto.
-      generalize h_CM_eval_expr2.
-      !intro.
-      eapply h_aligned_m in h_CM_eval_expr3.
-
-      destruct h_CM_eval_expr3.
-      subst.
-      assert (heq_ld_m:Memory.Mem.loadv AST.Mint32 m (Values.Vptr x Int.zero) = Some v). {
-        simpl.
-        erewrite <- (Memory.Mem.load_store_other);eauto. }
-      red in h_aligned_m.
-      eapply (h_aligned_m _ (S δ_lvl)).
-      simpl.
-      econstructor;eauto.
-  Qed.
-
-
-  
-
-  
-
-  
-Set Printing Width 78.
-
-  Lemma assignment_preserve_stack_match :
-    forall stbl CE g locenv stkptr s m a chk id id_t e_v e_t_v idaddr s' m' ,
-      increasing_orderG CE ->
-      Forall (λ otherfrm : CompilEnv.frame, increasing_order_fr otherfrm) CE ->
-      (∀ (id : idnum) (δ : CompilEnv.V),
-          CompilEnv.fetchG id CE = Some δ → 0 <= δ ∧ δ < Integers.Int.modulus) ->
-      (* translating the variabe to a Cminor load address *)
-      transl_variable stbl CE a id = OK id_t ->
-      (* translating the value, we may need a overflow hypothesis on e_v/e_t_v *)
-      transl_value e_v e_t_v ->
-      (* Evaluating var address in Cminor *)
-      Cminor.eval_expr g stkptr locenv m id_t idaddr ->
-      (* Size of variable in Cminor memorry *)
-      compute_chnk stbl (E_Identifier a id) = OK chk ->
-      (* the two storing operation maintain match_env *)
-      storeUpdate stbl s (E_Identifier a id) e_v (Normal s') ->
-      Memory.Mem.storev chk m idaddr e_t_v = Some m' ->
-      match_env stbl s CE stkptr locenv g m ->
-      stack_match stbl s' CE stkptr locenv g m'.
-  Proof.
-    intros until m'. (* if !intros. then id-t get renamed int id_t0? *)
-    !intros.
-    rename H1 into h_fetch_bounds.
-    !inversion h_match_env.
-    (* Getting rid of erronous cases *)
-    !functional inversion heq_transl_variable.
-    rename m'0 into lvl_max.
-    (* done *)
-    (* getting rid of erroneous storev parameter *)
-    rewrite <- cm_storev_ok in heq_storev_e_t_v.
-    !functional inversion heq_storev_e_t_v;subst.
-    set (loads_id:=(build_loads (lvl_max - lvl_id) δ_id)) in *.
-    rewrite cm_storev_ok in *.
-    (* done *)
-    assert (h_ofs_nonzero:4 <= Int.unsigned ofs). {
-      eapply eval_build_loads_offset_non_null_var;eauto. }
-
-    unfold stack_match.
-    !intros other_nme other_val addrof_other_nme load_addrof_other_nme type_other_nme cm_typ_other_nme.
-    (* id can already be evaluated in s *)
-    destruct (h_stk_cmpl_s_CE _ _ _ heq_transl_variable) as [v_id_prev h_eval_name_id_val_prev].
-    set (nme:=(E_Identifier a id)) in *.
-    (* done *)
-    (* Getting rid of erronous cases *)
-    !functional inversion heq_transl_name.
+Lemma transl_variable_inj :
+  forall CE stbl a₁ a₂ id₁ id₂ k₁ k₂ δ₁ δ₂,
+    (* Frame are numbered with different (increasing) numers *)
+    increasing_orderG CE ->
+    (* In each frame, stacks are also numbered with (increasing) numbers *)
+    List.Forall (fun otherfrm => increasing_order_fr otherfrm) CE ->
+    (forall id δ, CompilEnv.fetchG id CE = Some δ -> 0 <= δ ∧ δ < Integers.Int.modulus) ->
+    (* translating the variabe to a Cminor load address *)
+    transl_variable stbl CE a₁ id₁ = OK (build_loads k₁ δ₁) ->
+    (* translating the variabe to a Cminor load address *)
+    transl_variable stbl CE a₂ id₂ = OK   (build_loads k₂ δ₂) ->
+    id₁ <> id₂ ->
+    (k₁ <> k₂ \/ δ₁<> δ₂).
+Proof.
+  !intros.
+  match goal with
+  | H: appcontext [(0 <= _) ∧ (_ < Integers.Int.modulus)] |- _ => rename H into h_bound_CE
+  end.
+  unfold transl_variable in *.
+  destruct (CompilEnv.fetchG id₁ CE) eqn:h₁;simpl in *;try discriminate.
+  destruct (CompilEnv.fetchG id₂ CE) eqn:h₂;simpl in *;try discriminate.
+  destruct (CompilEnv.frameG id₁ CE) eqn:h₁';simpl in *;try discriminate.
+  destruct (CompilEnv.frameG id₂ CE) eqn:h₂';simpl in *;try discriminate.
+  destruct f.
+  destruct f0.
+  assert (hh:=CEfetchG_inj _ _ _ h_incr_orderG_CE h_forall_CE _ _ _ _ _ _  h₁ h₂ h₁' h₂' hneq).
+  destruct (CompilEnv.level_of_top CE) eqn:hlvlofCE.
+  - (* remember here refrain inversion to bizarrely unfold too much. *)
+    remember (build_loads (s3 - s1) t0) as fooo.
+    remember (build_loads (s3 - s) t) as fooo'.
+    inversion heq_transl_variable as [heqfoo].
+    inversion heq_transl_variable0 as [heqfoo'].
+    clear heq_transl_variable heq_transl_variable0.
     subst.
-    rename id0 into other_id.
-    set (other_nme:=(E_Identifier astnum other_id)) in *.
-(*     simpl in *. *)
-    (* done *)
-    (* other_nme can already be evaluated in s *)
-    destruct (h_stk_cmpl_s_CE _ _ _ heq_transl_variable0)
-      as [v_other_id_prev h_eval_name_other_id_val_prev].
-    (* done *)
-    destruct (h_stk_mtch_s_m
-                _ _ _ _ _ _ h_eval_name_other_id_val_prev
-                heq_type_of_name heq_transl_name heq_transl_type heq_make_load)
-      as [ cm_v [tr_val_v_other cm_eval_m_v_other]].
-    assert (h_tr_exp_other:
-              transl_expr stbl CE (E_Name 1%nat (E_Identifier astnum other_id))
-                          =: load_addrof_other_nme). {
+    apply build_loads_inj in heqfoo.
+    apply build_loads_inj in heqfoo'.
+    !destruct heqfoo.
+    !destruct heqfoo'.
+    subst.
+    !destruct hh.
+    + left.
+      eapply minus_same_neq;eauto.
+      eapply increase_order_level_of_top_ge;eauto.
+      eapply increase_order_level_of_top_ge;eauto.
+    + repeat rewrite Integers.Int.Z_mod_modulus_eq in *.
+      rewrite Coqlib.Zmod_small in *;eauto.
+      subst.
+      right.
+      intro abs.
+      subst.
+      apply hneq0;reflexivity.
+  - discriminate.
+Qed.
+
+Lemma transl_variable_astnum:
+  forall stbl CE astnum id' addrof_nme,
+    transl_variable stbl CE astnum id' = OK addrof_nme
+    -> forall a,transl_variable stbl CE a id' = transl_variable stbl CE astnum id'.
+Proof.
+  !intros.
+  unfold transl_variable.
+  !functional inversion heq_transl_variable.
+  rewrite  heq_CEfetchG_id'_CE, heq_CEframeG_id'_CE, heq_lvloftop_CE_m'.
+  reflexivity.
+Qed.
+
+
+
+Lemma compute_chk_32 :
+  forall stbl t,
+    compute_chnk_of_type stbl t = OK AST.Mint32
+    -> transl_type stbl t = OK (Ctypes.Tint Ctypes.I32 Ctypes.Signed Ctypes.noattr).
+Proof.
+  !intros.
+  functional inversion heq;subst;simpl.
+  - functional inversion H;simpl.
+    reflexivity.
+  - functional inversion H;simpl.
+    reflexivity.
+Qed.
+
+
+Notation " x =: y" := (x = OK y) (at level 90).
+Notation " x =! y" := (x = Error y) (at level 120).
+
+Ltac simplify_do :=
+  repeat progress
+         (match goal with
+          | H: context [do _ <- ?e ; _] , H': ?e = _ |- _ =>
+            rewrite H' in H;simpl in H
+                          | H': ?e = _ |- context [do _ <- ?e ; _]  =>
+                            rewrite H';simpl
+          end).
+
+
+(* Well-formedness of the chained stack: store never modify the
+     address of a variable. Reason: since variable addresses are
+     expressions of the form ((Load(Load(...(Load 0))))+δ) with δ >= 4
+     and that stores never touch the addresses 0, variables addresses
+     never change. *)
+Lemma wf_chain_load'2:forall g locenv stkptr chk m m' b ofs e_t_v
+                             vaddr,
+    Mem.storev chk m (Values.Vptr b ofs) e_t_v = Some m'
+    -> (stack_localstack_aligned locenv g m)
+    -> (4 <= (Int.unsigned ofs))(*forall n, Integers.Int.repr n = ofs -> 4 <= n*)
+    -> forall lvl,
+        let load_id := build_loads_ lvl in
+        Cminor.eval_expr g stkptr locenv m' load_id vaddr
+        -> Cminor.eval_expr g stkptr locenv m load_id vaddr.
+Proof.
+  !intros.
+  rename H1 into h_ofs_non_zero.
+  simpl in *.
+  subst load_id.
+  generalize dependent vaddr.
+  induction lvl;!intros;simpl in *.
+  - !inversion h_CM_eval_expr;econstructor;eauto.
+  - !invclear h_CM_eval_expr.
+    assert (h_CM_eval_expr_on_m:Cminor.eval_expr g stkptr locenv m (build_loads_ lvl) vaddr0). { eapply IHlvl; eauto. }
+                                                                                               econstructor.
+    + eassumption.
+    + destruct vaddr0;simpl in *;try discriminate.
+      rewrite <- heq.
+      symmetry.
+      eapply Mem.load_store_other;eauto.
+      right.
+      left.
       simpl.
-      simpl in heq_type_of_name.
-      rewrite heq_transl_variable0, heq_type_of_name.
-      unfold value_at_addr.
-      rewrite heq_transl_type;simpl.
-      assumption. }
-    !destruct (Nat.eq_dec id other_id).
-    - subst nme. (* same variable ==> result is the value just stored *)
-      subst other_nme.
-      subst other_id.
-      simpl in heq_type_of_name.
-      assert (chk = AST.Mint32). {
-        rewrite compute_chnk_ok in heq_compute_chnk.
-        !functional inversion heq_compute_chnk;subst;auto. }
-      simpl in heq_compute_chnk.
-      unfold compute_chnk_id in heq_compute_chnk.
-      rewrite heq_type_of_name in heq_compute_chnk.
-      lazy beta iota delta [bind] in heq_compute_chnk.
-      rewrite (transl_variable_astnum _ _ _ _ _ heq_transl_variable0 a) in *.
-      rewrite heq_transl_variable0 in heq_transl_variable.
-      !invclear heq_transl_variable.
-      !assert (e_v = other_val). { eapply storeUpdate_id_ok_same_eval_name ;eauto. }
-      subst other_val.
-      exists e_t_v;split;auto.
-      !functional inversion heq_make_load;subst.
-      eapply eval_Eload with (Values.Vptr b ofs).
-      * { eapply wf_chain_load_var with (1:= heq_storev_e_t_v);eauto.
-          - eapply wf_chain_load_aligned;eauto. }
-      * simpl.
-        (* Should be ok by well typedness of the chained stack wrt
+      transitivity 4.
+      * !destruct (h_aligned_g_m _ _ _ h_CM_eval_expr_on_m).
+        !invclear heq.
+        !invclear heq0.
+        vm_compute.
+        intro abs;discriminate.
+      * apply h_ofs_non_zero.
+Qed.
+
+(* Well-formedness of the chained stack: store never modify the
+     address of a variable. Reason: since variable addresses are
+     expressions of the form ((Load(Load(...(Load 0))))+δ) with δ >= 4
+     and that stores never touch the addresses 0, variables addresses
+     never change. *)
+Lemma wf_chain_load'3:forall g locenv stkptr chk m m' b ofs e_t_v
+                             vaddr,
+    Mem.storev chk m (Values.Vptr b ofs) e_t_v = Some m'
+    -> stack_localstack_aligned locenv g m'
+    -> (4 <= (Int.unsigned ofs))(*forall n, Integers.Int.repr n = ofs -> 4 <= n*)
+    -> forall lvl,
+        let load_id := build_loads_ lvl in
+        Cminor.eval_expr g stkptr locenv m load_id vaddr
+        -> Cminor.eval_expr g stkptr locenv m' load_id vaddr.
+Proof.
+  !intros.
+  rename H1 into h_ofs_non_zero.
+  simpl in *.
+  subst load_id.
+  generalize dependent vaddr.
+  induction lvl;!intros;simpl in *.
+  - !inversion h_CM_eval_expr;econstructor;eauto.
+  - !invclear h_CM_eval_expr.
+    assert (h_CM_eval_expr_on_m':Cminor.eval_expr g stkptr locenv m' (build_loads_ lvl) vaddr0). { eapply IHlvl; eauto. }
+                                                                                                 econstructor.
+    + eassumption.
+    + destruct vaddr0;simpl in *;try discriminate.
+      rewrite <- heq.
+      eapply Mem.load_store_other;eauto.
+      right.
+      left.
+      simpl.
+      transitivity 4.
+      * !destruct (h_aligned_g_m' _ _ _ h_CM_eval_expr_on_m').
+        !invclear heq.
+        !invclear heq0.
+        vm_compute.
+        intro abs;discriminate.
+      * apply h_ofs_non_zero.
+Qed.
+
+
+Lemma wf_chain_load'':forall g locenv stkptr chk m m' b ofs e_t_v
+                             vaddr,
+    Mem.storev chk m (Values.Vptr b ofs) e_t_v = Some m'
+    -> (stack_localstack_aligned locenv g m)
+    -> (stack_localstack_aligned locenv g m')
+    -> (4 <= (Int.unsigned ofs))(*forall n, Integers.Int.repr n = ofs -> 4 <= n*)
+    -> forall lvl,
+        let load_id := build_loads_ lvl in
+        Cminor.eval_expr g stkptr locenv m' load_id vaddr
+        <-> Cminor.eval_expr g stkptr locenv m load_id vaddr.
+Proof.
+  intros g locenv stkptr chk m m' b ofs e_t_v vaddr H H0 H1 H2 lvl load_id.
+  split;intro .
+  - eapply wf_chain_load'2 ;eauto.
+  - eapply wf_chain_load'3 ;eauto.
+Qed.
+
+(* Well-formedness of the chained stack: store never modify the
+     address of a variable. Reason: since variable addresses are
+     expressions of the form ((Load(Load(...(Load 0))))+δ) with δ >= 4
+     and that stores never touch the addresses 0, variables addresses
+     never change. *)
+Lemma wf_chain_load':forall g locenv stkptr chk m m' b ofs e_t_v
+                            vaddr,
+    Mem.storev chk m (Values.Vptr b ofs) e_t_v = Some m'
+    -> (stack_localstack_aligned locenv g m')
+    -> (4 <= (Int.unsigned ofs))(*forall n, Integers.Int.repr n = ofs -> 4 <= n*)
+    -> forall lvl δ_lvl,
+        let load_id := build_loads lvl δ_lvl in
+        Cminor.eval_expr g stkptr locenv m load_id vaddr
+        -> Cminor.eval_expr g stkptr locenv m' load_id vaddr.
+Proof.
+  !intros.
+  rename H1 into h_ofs_non_zero.
+  simpl in *.
+  unfold build_loads in *.
+  !invclear h_CM_eval_expr_load_id.
+  econstructor;eauto.
+  Focus 2.
+  { inversion h_CM_eval_expr;econstructor;eauto. }
+  Unfocus.
+  eapply wf_chain_load'3;eauto.
+Qed.
+
+(* Well-formedness of the chained stack: store never modify the
+     address of a variable. Reason: since variable addresses are
+     expressions of the form ((Load(Load(...(Load 0))))+δ) with δ >= 4
+     and that stores never touch the addresses 0, variables addresses
+     never change. *)
+Lemma wf_chain_load'_2:forall g locenv stkptr chk m m' b ofs e_t_v
+                              vaddr,
+    Mem.storev chk m (Values.Vptr b ofs) e_t_v = Some m'
+    -> (stack_localstack_aligned locenv g m)
+    -> (4 <= (Int.unsigned ofs))(*forall n, Integers.Int.repr n = ofs -> 4 <= n*)
+    -> forall lvl δ_lvl,
+        let load_id := build_loads lvl δ_lvl in
+        Cminor.eval_expr g stkptr locenv m' load_id vaddr
+        -> Cminor.eval_expr g stkptr locenv m load_id vaddr.
+Proof.
+  !intros.
+  rename H1 into h_ofs_non_zero.
+  simpl in *.
+  unfold build_loads in *.
+  !invclear h_CM_eval_expr_load_id.
+  econstructor;eauto.
+  Focus 2.
+  { inversion h_CM_eval_expr;econstructor;eauto. }
+  Unfocus.
+  eapply wf_chain_load'2;eauto.
+Qed.
+
+(* Well-formedness of the chained stack: store never modify the
+     address of a variable. Reason: since variable addresses are
+     expressions of the form ((Load(Load(...(Load 0))))+δ) with δ >= 4
+     and that stores never touch the addresses 0, variables addresses
+     never change. *)
+Lemma wf_chain_load_var:forall stbl CE g locenv stkptr astnum chk m m' b ofs e_t_v
+                               id load_id vaddr,
+    Mem.storev chk m (Values.Vptr b ofs) e_t_v = Some m'
+    -> (stack_localstack_aligned locenv g m')
+    -> (4 <= (Int.unsigned ofs))(*forall n, Integers.Int.repr n = ofs -> 4 <= n*)
+    -> transl_variable stbl CE astnum id =: load_id
+    -> Cminor.eval_expr g stkptr locenv m load_id vaddr
+    -> Cminor.eval_expr g stkptr locenv m' load_id vaddr.
+Proof.
+  !intros.
+  rename H1 into h_ofs_non_zero.
+  simpl in *.
+  !functional inversion heq_transl_variable;subst;clear heq_transl_variable.
+  rename m'0 into max_lvl.
+  set (δ_lvl:=(max_lvl - lvl_id)%nat) in *.
+  eapply wf_chain_load';eauto.
+Qed.
+
+(* Well-formedness of the chained stack: store never modify the
+     address of a variable. Reason: since variable addresses are
+     expressions of the form ((Load(Load(...(Load 0))))+δ) with δ >= 4
+     and that stores never touch the addresses 0, variables addresses
+     never change. *)
+Lemma wf_chain_load_var':forall stbl CE g locenv stkptr astnum chk m m' b ofs e_t_v
+                                id load_id vaddr,
+    Mem.storev chk m (Values.Vptr b ofs) e_t_v = Some m'
+    -> (stack_localstack_aligned locenv g m)
+    -> (4 <= (Int.unsigned ofs))(*forall n, Integers.Int.repr n = ofs -> 4 <= n*)
+    -> transl_variable stbl CE astnum id =: load_id
+    -> Cminor.eval_expr g stkptr locenv m' load_id vaddr
+    -> Cminor.eval_expr g stkptr locenv m load_id vaddr.
+Proof.
+  !intros.
+  rename H1 into h_ofs_non_zero.
+  simpl in *.
+  !functional inversion heq_transl_variable;subst;clear heq_transl_variable.
+  rename m'0 into max_lvl.
+  set (δ_lvl:=(max_lvl - lvl_id)%nat) in *.
+  eapply wf_chain_load'_2;eauto.
+Qed.
+
+
+(* INVARIANT OF STORE/STOREV: if we do not touch on addresses zero
+     of blocks, chaining variables all poitn to zero ofsets. *)
+Lemma wf_chain_load_aligned:forall g locenv chk m m' b ofs e_t_v,
+    Mem.storev chk m (Values.Vptr b ofs) e_t_v = Some m'
+    -> (4 <= (Int.unsigned ofs))
+    -> stack_localstack_aligned locenv g m
+    -> stack_localstack_aligned locenv g m'.
+Proof.
+  unfold stack_localstack_aligned at 2.
+  !intros.
+  revert g locenv chk m m' b ofs e_t_v heq_storev_e_t_v_m' H0 h_aligned_g_m b0 v h_CM_eval_expr.
+  destruct δ_lvl;simpl;!intros.
+  - rename h_aligned_g_m0 into h_aligned_m.
+    rename h_CM_eval_expr0 into h_CM_eval_expr.
+    edestruct (h_aligned_m b0 O v).
+    + simpl.
+      constructor.
+      !inversion h_CM_eval_expr.
+      assumption.
+    + eauto.
+  - rename h_aligned_g_m0 into h_aligned_m.
+    rename h_CM_eval_expr0 into h_CM_eval_expr.
+    !inversion h_CM_eval_expr.
+    generalize h_CM_eval_expr0.
+    !intro.
+    eapply wf_chain_load'2 in h_CM_eval_expr2;eauto.
+    generalize h_CM_eval_expr2.
+    !intro.
+    eapply h_aligned_m in h_CM_eval_expr3.
+
+    destruct h_CM_eval_expr3.
+    subst.
+    assert (heq_ld_m:Mem.loadv AST.Mint32 m (Values.Vptr x Int.zero) = Some v). {
+      simpl.
+      erewrite <- (Mem.load_store_other);eauto. }
+    red in h_aligned_m.
+    eapply (h_aligned_m _ (S δ_lvl)).
+    simpl.
+    econstructor;eauto.
+Qed.
+
+
+
+
+Lemma assignment_preserve_stack_match :
+  forall stbl CE g locenv stkptr s m a chk id id_t e_v e_t_v idaddr s' m' ,
+    increasing_orderG CE ->
+    Forall (λ otherfrm : CompilEnv.frame, increasing_order_fr otherfrm) CE ->
+    (∀ (id : idnum) (δ : CompilEnv.V),
+        CompilEnv.fetchG id CE = Some δ → 0 <= δ ∧ δ < Integers.Int.modulus) ->
+    (* translating the variabe to a Cminor load address *)
+    transl_variable stbl CE a id = OK id_t ->
+    (* translating the value, we may need a overflow hypothesis on e_v/e_t_v *)
+    transl_value e_v e_t_v ->
+    (* Evaluating var address in Cminor *)
+    Cminor.eval_expr g stkptr locenv m id_t idaddr ->
+    (* Size of variable in Cminor memorry *)
+    compute_chnk stbl (E_Identifier a id) = OK chk ->
+    (* the two storing operation maintain match_env *)
+    storeUpdate stbl s (E_Identifier a id) e_v (Normal s') ->
+    Mem.storev chk m idaddr e_t_v = Some m' ->
+    match_env stbl s CE stkptr locenv g m ->
+    stack_match stbl s' CE stkptr locenv g m'.
+Proof.
+  intros until m'. (* if !intros. then id-t get renamed int id_t0? *)
+  !intros.
+  rename H1 into h_fetch_bounds.
+  !inversion h_match_env.
+  (* Getting rid of erronous cases *)
+  !functional inversion heq_transl_variable.
+  rename m'0 into lvl_max.
+  (* done *)
+  (* getting rid of erroneous storev parameter *)
+  rewrite <- cm_storev_ok in heq_storev_e_t_v_m'.
+  !functional inversion heq_storev_e_t_v_m';subst.
+  set (loads_id:=(build_loads (lvl_max - lvl_id) δ_id)) in *.
+  rewrite cm_storev_ok in *.
+  (* done *)
+  assert (h_ofs_nonzero:4 <= Int.unsigned ofs). {
+    eapply eval_build_loads_offset_non_null_var;eauto. }
+
+  unfold stack_match.
+  !intros other_nme other_val addrof_other_nme load_addrof_other_nme type_other_nme cm_typ_other_nme.
+  (* id can already be evaluated in s *)
+  destruct (h_stk_cmpl_s_CE _ _ _ heq_transl_variable) as [v_id_prev h_eval_name_id_val_prev].
+  set (nme:=(E_Identifier a id)) in *.
+  (* done *)
+  (* Getting rid of erronous cases *)
+  !functional inversion heq_transl_name.
+  subst.
+  rename id0 into other_id.
+  set (other_nme:=(E_Identifier astnum other_id)) in *.
+  (*     simpl in *. *)
+  (* done *)
+  (* other_nme can already be evaluated in s *)
+  destruct (h_stk_cmpl_s_CE _ _ _ heq_transl_variable0)
+    as [v_other_id_prev h_eval_name_other_id_val_prev].
+  (* done *)
+  destruct (h_stk_mtch_s_m
+              _ _ _ _ _ _ h_eval_name_other_id_val_prev
+              heq_type_of_name heq_transl_name heq_transl_type heq_make_load)
+    as [ cm_v [tr_val_v_other cm_eval_m_v_other]].
+  assert (h_tr_exp_other:
+            transl_expr stbl CE (E_Name 1%nat (E_Identifier astnum other_id))
+                        =: load_addrof_other_nme). {
+    simpl.
+    simpl in heq_type_of_name.
+    rewrite heq_transl_variable0, heq_type_of_name.
+    unfold value_at_addr.
+    rewrite heq_transl_type;simpl.
+    assumption. }
+  !destruct (Nat.eq_dec id other_id).
+  - subst nme. (* same variable ==> result is the value just stored *)
+    subst other_nme.
+    subst other_id.
+    simpl in heq_type_of_name.
+    assert (chk = AST.Mint32). {
+      rewrite compute_chnk_ok in heq_compute_chnk.
+      !functional inversion heq_compute_chnk;subst;auto. }
+    simpl in heq_compute_chnk.
+    unfold compute_chnk_id in heq_compute_chnk.
+    rewrite heq_type_of_name in heq_compute_chnk.
+    lazy beta iota delta [bind] in heq_compute_chnk.
+    rewrite (transl_variable_astnum _ _ _ _ _ heq_transl_variable0 a) in *.
+    rewrite heq_transl_variable0 in heq_transl_variable.
+    !invclear heq_transl_variable.
+    !assert (e_v = other_val). { eapply storeUpdate_id_ok_same_eval_name ;eauto. }
+                               subst other_val.
+    exists e_t_v;split;auto.
+    !functional inversion heq_make_load;subst.
+    eapply eval_Eload with (Values.Vptr b ofs).
+    * { eapply wf_chain_load_var with (1:= heq_storev_e_t_v_m');eauto.
+        - eapply wf_chain_load_aligned;eauto. }
+    * simpl.
+      (* Should be ok by well typedness of the chained stack wrt
            stbl (see hyp on compute_chk). *)
-        (* assert (chunk = AST.chunk_of_type t). {
+      (* assert (chunk = AST.chunk_of_type t). {
            rewrite cmtype_chk with (1:=heq_transl_type) (2:=heq_opttype) (3:=heq0).
            reflexivity. } *)
-        assert (chunk = AST.Mint32). {
-          !functional inversion heq_transl_type;subst;simpl in h_access_mode_cm_typ_other_nme.
-          - inversion h_access_mode_cm_typ_other_nme;auto.
-          - inversion h_access_mode_cm_typ_other_nme;auto. }
-        subst.
-        erewrite (Memory.Mem.load_store_same _ _ _ _ _ _ heq_store_e_t_v) .
-        { destruct e_t_v;auto;destruct e_v;simpl in *;try discriminate; now inversion heq_transl_value. }
-        
-    - (* loading a different variable id' than the one stored id.
+      assert (chunk = AST.Mint32). {
+        !functional inversion heq_transl_type;subst;simpl in h_access_mode_cm_typ_other_nme.
+        - inversion h_access_mode_cm_typ_other_nme;auto.
+        - inversion h_access_mode_cm_typ_other_nme;auto. }
+      subst.
+      erewrite (Mem.load_store_same _ _ _ _ _ _ heq_store_e_t_v_m') .
+      { destruct e_t_v;auto;destruct e_v;simpl in *;try discriminate; now inversion heq_transl_value. }
+      
+  - (* loading a different variable id' than the one stored id.
          2 steps: first prove that the addresses of id' and id did
          not change (the translated expressions did not change + the
          chained stack did not change either), and thus remain
          different, then conclude that the value stored in id' did
          not change. *)
-      !assert (chk = AST.Mint32). {
-        rewrite function_utils.compute_chnk_ok in heq_compute_chnk.
-        functional inversion heq_compute_chnk; reflexivity. }
+    !assert (chk = AST.Mint32). {
+      rewrite function_utils.compute_chnk_ok in heq_compute_chnk.
+      functional inversion heq_compute_chnk; reflexivity. }
 
-      assert (v_other_id_prev = other_val). { eapply storeUpdate_id_ok_others_eval_name ;eauto. }
-      subst.
-      exists cm_v.
-      split;auto.
-      assert (h_aligned_m' : stack_localstack_aligned locenv g m'). {
-        eapply wf_chain_load_aligned;eauto. }
-      !functional inversion heq_make_load;subst.
-      !inversion cm_eval_m_v_other.
-      generalize (wf_chain_load_var _ _ _ _ _ _ _ _ _ _ _ _ _ _ _
-                                heq_storev_e_t_v h_aligned_m'
-                                h_ofs_nonzero heq_transl_variable0
-                                h_CM_eval_expr_addrof_other_nme).
-      !intro.
-      econstructor.
-      + eassumption.
-      + destruct vaddr; try discriminate;simpl in *.
-        clear h_tr_exp_other.
-        erewrite Memory.Mem.load_store_other;[now eassumption| now eassumption | ].
-        subst nme other_nme.
-        unfold compute_chnk_id in heq_compute_chnk.
-        destruct (fetch_var_type id stbl) eqn:heq_fetchvartyp;try discriminate.
-        simpl in heq_compute_chnk.
+    assert (v_other_id_prev = other_val). { eapply storeUpdate_id_ok_others_eval_name ;eauto. }
+                                          subst.
+    exists cm_v.
+    split;auto.
+    assert (h_aligned_m' : stack_localstack_aligned locenv g m'). {
+      eapply wf_chain_load_aligned;eauto. }
+    !functional inversion heq_make_load;subst.
+    !inversion cm_eval_m_v_other.
+    generalize (wf_chain_load_var _ _ _ _ _ _ _ _ _ _ _ _ _ _ _
+                                  heq_storev_e_t_v_m' h_aligned_m'
+                                  h_ofs_nonzero heq_transl_variable0
+                                  h_CM_eval_expr_addrof_other_nme).
+    !intro.
+    econstructor.
+    + eassumption.
+    + destruct vaddr; try discriminate;simpl in *.
+      clear h_tr_exp_other.
+      erewrite Mem.load_store_other;[now eassumption| now eassumption | ].
+      subst nme other_nme.
+      unfold compute_chnk_id in heq_compute_chnk.
+      destruct (fetch_var_type id stbl) eqn:heq_fetchvartyp;try discriminate.
+      simpl in heq_compute_chnk.
 
-        assert (heq_tr_type_id:transl_type stbl t = OK (Ctypes.Tint Ctypes.I32 Ctypes.Signed Ctypes.noattr)). {
-          apply compute_chk_32;auto. }
-        unfold stack_separate in h_separate_CE_m.
-        { eapply h_separate_CE_m with (nme:=(E_Identifier a id))
-                             (nme':=(E_Identifier astnum other_id))
-                             (k₂ := b0) (k₁:=b); clear h_separate_CE_m;simpl;try eassumption;auto.
-          intro abs.
-          inversion abs;subst;try discriminate.
-          elim hneq;reflexivity. }
-  Qed.
-
-
-  Lemma storev_inv : forall nme_chk m nme_t_addr e_t_v m',
-      Memory.Mem.storev nme_chk m nme_t_addr e_t_v = Some m'
-      -> exists b ofs, nme_t_addr = Values.Vptr b ofs.
-  Proof.
-    !intros.
-    destruct nme_t_addr; try discriminate.
-    eauto.
-  Qed.        
-
-  Lemma transl_name_OK_inv : forall stbl CE nme nme_t,
-      transl_name stbl CE nme = OK nme_t
-      -> exists astnum id, (transl_variable stbl CE astnum id =  OK nme_t /\ nme = E_Identifier astnum id).
-  Proof.
-    !intros stbl CE nme nme_t H.
-    functional inversion H.
-    eauto.
-  Qed.
- 
-  Lemma assignment_preserve_stack_complete :
-    forall stbl CE g locenv stkptr s m a chk id id_t e_v e_t_v idaddr s' m' ,
-      increasing_orderG CE ->
-      Forall (λ otherfrm : CompilEnv.frame, increasing_order_fr otherfrm) CE ->
-      (∀ (id : idnum) (δ : CompilEnv.V),
-          CompilEnv.fetchG id CE = Some δ → 0 <= δ ∧ δ < Integers.Int.modulus) ->
-      (* translating the variabe to a Cminor load address *)
-      transl_variable stbl CE a id = OK id_t ->
-      (* translating the value, we may need a overflow hypothesis on e_v/e_t_v *)
-      transl_value e_v e_t_v ->
-      (* Evaluating var address in Cminor *)
-      Cminor.eval_expr g stkptr locenv m id_t idaddr ->
-      (* Size of variable in Cminor memorry *)
-      compute_chnk stbl (E_Identifier a id) = OK chk ->
-      (* the two storing operation maintain match_env *)
-      storeUpdate stbl s (E_Identifier a id) e_v (Normal s') ->
-      Memory.Mem.storev chk m idaddr e_t_v = Some m' ->
-      stack_complete stbl s CE ->
-      stack_complete stbl s' CE.
-  Proof.
-    !intros.
-    red.
-    !intros.
-    !destruct (Nat.eq_dec nme id).
-    - subst.
-      exists e_v.
-      constructor.
-      eapply storeUpdate_id_ok_same;eauto.
-    - red in h_stk_cmpl_s_CE.
-      destruct h_stk_cmpl_s_CE with (1:=heq_transl_variable0).
-      exists x.
-      constructor.
-      !invclear H.
-      erewrite <- storeUpdate_id_ok_others.
-      + eassumption.
-      + eassumption.
-      + apply not_eq_sym;assumption.
-  Qed.
-
-  Lemma assignment_preserve_stack_separate :
-    forall stbl CE g locenv stkptr s m a chk id id_t e_v e_t_v idaddr s' m' ,
-      increasing_orderG CE ->
-      Forall (λ otherfrm : CompilEnv.frame, increasing_order_fr otherfrm) CE ->
-      (∀ (id : idnum) (δ : CompilEnv.V),
-          CompilEnv.fetchG id CE = Some δ → 0 <= δ ∧ δ < Integers.Int.modulus) ->
-      (* translating the variabe to a Cminor load address *)
-      transl_variable stbl CE a id = OK id_t ->
-      (* translating the value, we may need a overflow hypothesis on e_v/e_t_v *)
-      transl_value e_v e_t_v ->
-      (* Evaluating var address in Cminor *)
-      Cminor.eval_expr g stkptr locenv m id_t idaddr ->
-      (* Size of variable in Cminor memorry *)
-      compute_chnk stbl (E_Identifier a id) = OK chk ->
-      (* the two storing operation maintain match_env *)
-      storeUpdate stbl s (E_Identifier a id) e_v (Normal s') ->
-      Memory.Mem.storev chk m idaddr e_t_v = Some m' ->
-      match_env stbl s CE stkptr locenv g m ->
-      stack_separate stbl CE stkptr locenv g m'.
-  Proof.
-    !intros.
-    red.
-    !intros.
-    !destruct h_match_env.
-    decompose [ex] (storev_inv _ _ _ _ _ heq_storev_e_t_v);subst.
-    !functional inversion heq_transl_name;subst.
-    generalize heq_transl_name0.
-    intro h_transl_name_remember.
-    functional inversion h_transl_name_remember.
-    eapply wf_chain_load_var' with (m:=m) in h_CM_eval_expr_addrof_nme.
-    - eapply wf_chain_load_var' with (m:=m) in h_CM_eval_expr_addrof_nme'.
-      + eapply h_separate_CE_m with (1:=heq_type_of_name0);eauto.
-      + eassumption.
-      + assumption.
-      + eapply eval_build_loads_offset_non_null_var with (4:=h_CM_eval_expr_id_t);eauto.
-      + simpl in heq_transl_name.
-        eauto.
-    - eassumption.
-    - assumption.
-    - eapply eval_build_loads_offset_non_null_var with (4:=h_CM_eval_expr_id_t);eauto.
-    - eauto.
-  Qed.
-
-  Lemma assignment_preserve_stack_no_null_offset :
-    forall stbl CE g locenv stkptr s m a chk id id_t e_v e_t_v idaddr s' m' ,
-      increasing_orderG CE ->
-      Forall (λ otherfrm : CompilEnv.frame, increasing_order_fr otherfrm) CE ->
-      (∀ (id : idnum) (δ : CompilEnv.V),
-          CompilEnv.fetchG id CE = Some δ → 0 <= δ ∧ δ < Integers.Int.modulus) ->
-      (* translating the variabe to a Cminor load address *)
-      transl_variable stbl CE a id = OK id_t ->
-      (* translating the value, we may need a overflow hypothesis on e_v/e_t_v *)
-      transl_value e_v e_t_v ->
-      (* Evaluating var address in Cminor *)
-      Cminor.eval_expr g stkptr locenv m id_t idaddr ->
-      (* Size of variable in Cminor memorry *)
-      compute_chnk stbl (E_Identifier a id) = OK chk ->
-      (* the two storing operation maintain match_env *)
-      storeUpdate stbl s (E_Identifier a id) e_v (Normal s') ->
-      Memory.Mem.storev chk m idaddr e_t_v = Some m' ->
-      match_env stbl s CE stkptr locenv g m ->
-      stack_no_null_offset stbl CE.
-  Proof.
-    !intros.
-    destruct h_match_env.
-    assumption.
-  Qed.
-
-  Lemma assignment_preserve_stack_safe :
-    forall stbl CE g locenv stkptr s m a chk id id_t e_v e_t_v idaddr s' m' ,
-      increasing_orderG CE ->
-      Forall (λ otherfrm : CompilEnv.frame, increasing_order_fr otherfrm) CE ->
-      (∀ (id : idnum) (δ : CompilEnv.V),
-          CompilEnv.fetchG id CE = Some δ → 0 <= δ ∧ δ < Integers.Int.modulus) ->
-      (* translating the variabe to a Cminor load address *)
-      transl_variable stbl CE a id = OK id_t ->
-      (* translating the value, we may need a overflow hypothesis on e_v/e_t_v *)
-      transl_value e_v e_t_v ->
-      (* if e_v is an int, then it is not overflowing *)
-      (forall n, e_v = Int n -> do_overflow_check n (Normal (Int n))) ->
-      (* Evaluating var address in Cminor *)
-      Cminor.eval_expr g stkptr locenv m id_t idaddr ->
-      (* Size of variable in Cminor memorry *)
-      compute_chnk stbl (E_Identifier a id) = OK chk ->
-      (* the two storing operation maintain match_env *)
-      storeUpdate stbl s (E_Identifier a id) e_v (Normal s') ->
-      Memory.Mem.storev chk m idaddr e_t_v = Some m' ->
-      match_env stbl s CE stkptr locenv g m ->
-      safe_stack s'.
-  Proof.
-    !intros.
-    rename H1 into h_fetch_safe.
-    rename H4 into h_overf_e_v.
-    !destruct h_match_env.
-    !intros.
-    red.
-    !intros.
-    !destruct (Nat.eq_dec id0 id).
-    - subst.
-      apply h_overf_e_v.
-      erewrite storeUpdate_id_ok_same in heq_SfetchG;eauto.
-      inversion heq_SfetchG.
-      reflexivity.
-    - red in h_safe_stack_s.
-      apply h_safe_stack_s with (id:=id0);eauto.
-      erewrite storeUpdate_id_ok_others;eauto.
-  Qed.
+      assert (heq_tr_type_id:transl_type stbl t = OK (Ctypes.Tint Ctypes.I32 Ctypes.Signed Ctypes.noattr)). {
+        apply compute_chk_32;auto. }
+      unfold stack_separate in h_separate_CE_m.
+      { eapply h_separate_CE_m with (nme:=(E_Identifier a id))
+                                      (nme':=(E_Identifier astnum other_id))
+                                      (k₂ := b0) (k₁:=b); clear h_separate_CE_m;simpl;try eassumption;auto.
+        intro abs.
+        inversion abs;subst;try discriminate.
+        elim hneq;reflexivity. }
+Qed.
 
 
-Set Printing Width 78.
+Lemma storev_inv : forall nme_chk m nme_t_addr e_t_v m',
+    Mem.storev nme_chk m nme_t_addr e_t_v = Some m'
+    -> exists b ofs, nme_t_addr = Values.Vptr b ofs.
+Proof.
+  !intros.
+  destruct nme_t_addr; try discriminate.
+  eauto.
+Qed.        
+
+Lemma transl_name_OK_inv : forall stbl CE nme nme_t,
+    transl_name stbl CE nme = OK nme_t
+    -> exists astnum id, (transl_variable stbl CE astnum id =  OK nme_t /\ nme = E_Identifier astnum id).
+Proof.
+  !intros stbl CE nme nme_t H.
+  functional inversion H.
+  eauto.
+Qed.
+
+Lemma assignment_preserve_stack_complete :
+  forall stbl CE g locenv stkptr s m a chk id id_t e_v e_t_v idaddr s' m' ,
+    increasing_orderG CE ->
+    Forall (λ otherfrm : CompilEnv.frame, increasing_order_fr otherfrm) CE ->
+    (∀ (id : idnum) (δ : CompilEnv.V),
+        CompilEnv.fetchG id CE = Some δ → 0 <= δ ∧ δ < Integers.Int.modulus) ->
+    (* translating the variabe to a Cminor load address *)
+    transl_variable stbl CE a id = OK id_t ->
+    (* translating the value, we may need a overflow hypothesis on e_v/e_t_v *)
+    transl_value e_v e_t_v ->
+    (* Evaluating var address in Cminor *)
+    Cminor.eval_expr g stkptr locenv m id_t idaddr ->
+    (* Size of variable in Cminor memorry *)
+    compute_chnk stbl (E_Identifier a id) = OK chk ->
+    (* the two storing operation maintain match_env *)
+    storeUpdate stbl s (E_Identifier a id) e_v (Normal s') ->
+    Mem.storev chk m idaddr e_t_v = Some m' ->
+    stack_complete stbl s CE ->
+    stack_complete stbl s' CE.
+Proof.
+  !intros.
+  red.
+  !intros.
+  !destruct (Nat.eq_dec nme id).
+  - subst.
+    exists e_v.
+    constructor.
+    eapply storeUpdate_id_ok_same;eauto.
+  - red in h_stk_cmpl_s_CE.
+    destruct h_stk_cmpl_s_CE with (1:=heq_transl_variable0).
+    exists x.
+    constructor.
+    !invclear H.
+    erewrite <- storeUpdate_id_ok_others.
+    + eassumption.
+    + eassumption.
+    + apply not_eq_sym;assumption.
+Qed.
+
+Lemma assignment_preserve_stack_separate :
+  forall stbl CE g locenv stkptr s m a chk id id_t e_v e_t_v idaddr s' m' ,
+    increasing_orderG CE ->
+    Forall (λ otherfrm : CompilEnv.frame, increasing_order_fr otherfrm) CE ->
+    (∀ (id : idnum) (δ : CompilEnv.V),
+        CompilEnv.fetchG id CE = Some δ → 0 <= δ ∧ δ < Integers.Int.modulus) ->
+    (* translating the variabe to a Cminor load address *)
+    transl_variable stbl CE a id = OK id_t ->
+    (* translating the value, we may need a overflow hypothesis on e_v/e_t_v *)
+    transl_value e_v e_t_v ->
+    (* Evaluating var address in Cminor *)
+    Cminor.eval_expr g stkptr locenv m id_t idaddr ->
+    (* Size of variable in Cminor memorry *)
+    compute_chnk stbl (E_Identifier a id) = OK chk ->
+    (* the two storing operation maintain match_env *)
+    storeUpdate stbl s (E_Identifier a id) e_v (Normal s') ->
+    Mem.storev chk m idaddr e_t_v = Some m' ->
+    match_env stbl s CE stkptr locenv g m ->
+    stack_separate stbl CE stkptr locenv g m'.
+Proof.
+  !intros.
+  red.
+  !intros.
+  !destruct h_match_env.
+  decompose [ex] (storev_inv _ _ _ _ _ heq_storev_e_t_v_m');subst.
+  !functional inversion heq_transl_name;subst.
+  generalize heq_transl_name0.
+  intro h_transl_name_remember.
+  functional inversion h_transl_name_remember.
+  eapply wf_chain_load_var' with (m:=m) in h_CM_eval_expr_addrof_nme.
+  - eapply wf_chain_load_var' with (m:=m) in h_CM_eval_expr_addrof_nme'.
+    + eapply h_separate_CE_m with (1:=heq_type_of_name0);eauto.
+    + eassumption.
+    + assumption.
+    + eapply eval_build_loads_offset_non_null_var with (4:=h_CM_eval_expr_id_t);eauto.
+    + simpl in heq_transl_name.
+      eauto.
+  - eassumption.
+  - assumption.
+  - eapply eval_build_loads_offset_non_null_var with (4:=h_CM_eval_expr_id_t);eauto.
+  - eauto.
+Qed.
+
+Lemma assignment_preserve_stack_no_null_offset :
+  forall stbl CE g locenv stkptr s m a chk id id_t e_v e_t_v idaddr s' m' ,
+    increasing_orderG CE ->
+    Forall (λ otherfrm : CompilEnv.frame, increasing_order_fr otherfrm) CE ->
+    (∀ (id : idnum) (δ : CompilEnv.V),
+        CompilEnv.fetchG id CE = Some δ → 0 <= δ ∧ δ < Integers.Int.modulus) ->
+    (* translating the variabe to a Cminor load address *)
+    transl_variable stbl CE a id = OK id_t ->
+    (* translating the value, we may need a overflow hypothesis on e_v/e_t_v *)
+    transl_value e_v e_t_v ->
+    (* Evaluating var address in Cminor *)
+    Cminor.eval_expr g stkptr locenv m id_t idaddr ->
+    (* Size of variable in Cminor memorry *)
+    compute_chnk stbl (E_Identifier a id) = OK chk ->
+    (* the two storing operation maintain match_env *)
+    storeUpdate stbl s (E_Identifier a id) e_v (Normal s') ->
+    Mem.storev chk m idaddr e_t_v = Some m' ->
+    match_env stbl s CE stkptr locenv g m ->
+    stack_no_null_offset stbl CE.
+Proof.
+  !intros.
+  destruct h_match_env.
+  assumption.
+Qed.
+
+Lemma assignment_preserve_stack_safe :
+  forall stbl CE g locenv stkptr s m a chk id id_t e_v e_t_v idaddr s' m' ,
+    increasing_orderG CE ->
+    Forall (λ otherfrm : CompilEnv.frame, increasing_order_fr otherfrm) CE ->
+    (∀ (id : idnum) (δ : CompilEnv.V),
+        CompilEnv.fetchG id CE = Some δ → 0 <= δ ∧ δ < Integers.Int.modulus) ->
+    (* translating the variabe to a Cminor load address *)
+    transl_variable stbl CE a id = OK id_t ->
+    (* translating the value, we may need a overflow hypothesis on e_v/e_t_v *)
+    transl_value e_v e_t_v ->
+    (* if e_v is an int, then it is not overflowing *)
+    (forall n, e_v = Int n -> do_overflow_check n (Normal (Int n))) ->
+    (* Evaluating var address in Cminor *)
+    Cminor.eval_expr g stkptr locenv m id_t idaddr ->
+    (* Size of variable in Cminor memorry *)
+    compute_chnk stbl (E_Identifier a id) = OK chk ->
+    (* the two storing operation maintain match_env *)
+    storeUpdate stbl s (E_Identifier a id) e_v (Normal s') ->
+    Mem.storev chk m idaddr e_t_v = Some m' ->
+    match_env stbl s CE stkptr locenv g m ->
+    safe_stack s'.
+Proof.
+  !intros.
+  rename H1 into h_fetch_safe.
+  rename H4 into h_overf_e_v.
+  !destruct h_match_env.
+  !intros.
+  red.
+  !intros.
+  !destruct (Nat.eq_dec id0 id).
+  - subst.
+    apply h_overf_e_v.
+    erewrite storeUpdate_id_ok_same in heq_SfetchG_id0_s';eauto.
+    inversion heq_SfetchG_id0_s'.
+    reflexivity.
+  - red in h_safe_stack_s.
+    apply h_safe_stack_s with (id:=id0);eauto.
+    erewrite storeUpdate_id_ok_others;eauto.
+Qed.
+
+
 Lemma transl_stmt_ok :
   forall stbl CE  (stm:statement) (stm':Cminor.stmt),
-      increasing_orderG CE ->
-      Forall (λ otherfrm : CompilEnv.frame, increasing_order_fr otherfrm) CE ->
-      (∀ (id : idnum) (δ : CompilEnv.V),
-          CompilEnv.fetchG id CE = Some δ → 0 <= δ ∧ δ < Integers.Int.modulus) ->
+    invariant_compile CE ->
     transl_stmt stbl CE stm = (OK stm') ->
-    forall locenv (g:genv) (m:Memory.Mem.mem) (s:stack)
-           (s':stack) (spb:Values.block) ofs f,
+    forall locenv g m s s' spb ofs f,
       match_env stbl s CE (Values.Vptr spb ofs) locenv g m ->
       eval_stmt stbl s stm (Normal s') ->
       forall tr locenv' m' o,
@@ -2720,7 +2271,7 @@ Proof.
   - !invclear h_eval_stmt.
     !invclear h_exec_stmt.
     assumption.
-    (* assignment *)
+  (* assignment *)
   - rename e0 into e.
     rename x into e_t.
     rename x0 into nme_t.
@@ -2757,7 +2308,7 @@ Proof.
             eapply det_eval_expr;eauto. }
           subst x1.
           eassumption. }
-      * decomp (storev_inv _ _ _ _ _ heq_storev_v) ;subst.
+      * decomp (storev_inv _ _ _ _ _ heq_storev_v_m') ;subst.
         functional inversion heq_transl_name.
         eapply wf_chain_load_aligned;eauto.
         eapply eval_build_loads_offset_non_null_var;eauto.
@@ -2810,7 +2361,7 @@ Proof.
             eapply det_eval_expr;eauto. }
           subst x1.
           eassumption. }
-      * decomp (storev_inv _ _ _ _ _ heq_storev_v) ;subst.
+      * decomp (storev_inv _ _ _ _ _ heq_storev_v_m') ;subst.
         functional inversion heq_transl_name.
         eapply wf_chain_load_aligned;eauto.
         eapply eval_build_loads_offset_non_null_var;eauto.
@@ -2825,7 +2376,7 @@ Proof.
       * { decompose [and ex] (transl_name_OK_inv _ _ _ _ heq_transl_name);subst.
           eapply assignment_preserve_stack_safe;eauto.
           - decompose [ex and] (transl_expr_ok _ _ _ _ heq_tr_expr_e0 _ _ _ _ _ _
-                                             h_eval_expr h_match_env).
+                                               h_eval_expr h_match_env).
             assert (x1 = e_t_v). {
               eapply det_eval_expr;eauto. }
             subst x1.
@@ -2886,12 +2437,11 @@ Proof.
     rename s2 into stmt2.
     !invclear h_eval_stmt.
     !invclear h_exec_stmt.
-    + eapply IHr0 with (6:=h_eval_stmt); eauto. 
+    + eapply IHr0 with (4:=h_eval_stmt); eauto. 
     + (* o <> out_normal. is this possible?  *)
-      xxx.
-    
+      admit.
+
+      
 Admitted.
-
-
 
 
