compcert_utils.v
@@ -1,0 +1,58 @@
+Require Import LibHypsNaming spark2Cminor.
+Import ZArith Memory Cminor Integers.
+Open Scope Z_scope.
+
+Ltac rename_hyp1 h th :=
+  match th with
+    | ?min <= ?x and ?x < ?max => fresh "h_" x "_bounded_" min "_" max 
+    | ?min <= ?x and ?x < ?max => fresh "h_" x "_bounded_"
+    | ?min <= ?x and ?x < ?max => fresh "h_bounded"
+    | Ctypes.access_mode ?x = _ => fresh "h_access_mode_" x
+    | Ctypes.access_mode _ = _ => fresh "h_access_mode"
+    | Cminor.exec_stmt _ _ _ _ _ _ _ _ _ None  => fresh "h_exec_stmt_None"
+    | Cminor.exec_stmt _ _ _ _ _ _ _ _ _ _  => fresh "h_exec_stmt"
+    | Cminor.eval_constant _ _ _ = (Some _)  => fresh "h_eval_constant"
+    | Cminor.eval_constant _ _ _ = None  => fresh "h_eval_constant_None"
+    | Cminor.eval_expr _ _ _ _ ?x _ => fresh "h_CM_eval_expr_" x
+    | Cminor.eval_expr _ _ _ _ _ _ => fresh "h_CM_eval_expr"
+    | Mem.store ?chk ?m ?blk ?n ?v = None => fresh "heq_store_" v "_none"
+    | Mem.store ?chk ?m ?blk ?n ?v = Some ?m2 => fresh "heq_store_" v "_" m2
+    | Mem.store ?chk ?m ?blk ?n ?v = ?m2 => fresh "heq_store_" v "_" m2
+    | Mem.store ?chk ?m ?blk ?n ?v = ?m2 => fresh "heq_store_" v
+    | Mem.store ?chk ?m ?blk ?n ?v = ?m2 => fresh "heq_store"
+    | Mem.storev ?chk ?m ?vaddr ?v = None => fresh "heq_storev_" v "_none"
+    | Mem.storev ?chk ?m ?vaddr ?v = Some ?m2 => fresh "heq_storev_" v "_" m2
+    | Mem.storev ?chk ?m ?vaddr ?v = ?m2 => fresh "heq_storev_" v "_" m2
+    | Mem.storev ?chk ?m ?vaddr ?v = ?m2 => fresh "heq_storev_" v
+    | Mem.storev ?chk ?m ?vaddr ?v = ?m2 => fresh "heq_storev"
+  end.
+
+
+(* Auxiliary lemmas, should go in Compcert? *)
+Lemma repr_inj:
+  forall v1 v2,
+    Integers.Int.min_signed <= v1 <= Integers.Int.max_signed ->
+    Integers.Int.min_signed <= v2 <= Integers.Int.max_signed ->
+    Integers.Int.repr v1 = Integers.Int.repr v2 ->
+    v1 = v2.
+Proof.
+  intros v1 v2 hinbound1 hinboun2.
+  !intros.
+  assert (h: Integers.Int.signed(Integers.Int.repr v1)
+             = Integers.Int.signed(Integers.Int.repr v2)).
+  { rewrite heq. reflexivity. }
+  rewrite Integers.Int.signed_repr in h;auto.
+  rewrite Integers.Int.signed_repr in h;auto.
+Qed.
+
+Lemma repr_inj_neq:
+  forall v1 v2,
+    Integers.Int.min_signed <= v1 <= Integers.Int.max_signed ->
+    Integers.Int.min_signed <= v2 <= Integers.Int.max_signed ->
+    v1 <> v2 -> 
+    Integers.Int.repr v1 <> Integers.Int.repr v2.
+Proof.
+  intros v1 v2 hinbound1 hinboun2 hneq.
+  intro abs.
+  apply repr_inj in abs;auto.
+Qed.
