more_stdlib.v
@@ -1,0 +1,105 @@
+Require Import LibHypsNaming Sorted ZArith.
+
+(* All elements of a sorted list are smaller or equal to the first
+   element. If the ordering is reflexive. *)
+Lemma increasing_order_In A : forall ord (stk:list A) (hd:A),
+    StronglySorted ord (hd::stk) ->
+    List.Forall (fun elt => elt = hd \/ ord hd elt) (hd::stk).
+Proof.
+  !intros.
+  !inversion H.
+  constructor 2.
+  - left;reflexivity.
+  - apply List.Forall_forall.
+    !intros.
+    right.
+    rewrite List.Forall_forall in H3.
+    auto.
+Qed.
+
+Open Scope Z_scope.
+
+
+Lemma neq_sym A :  forall x y : A, (x = y -> False) -> y = x -> False.
+Proof.
+  auto.
+Qed.
+
+Add Parametric Relation A: A (fun x y : A => x <> y)
+    symmetry proved by (neq_sym A)
+as toto.
+
+(* FIXME: replace Z(n)eq_bool (which seems more or less deprecated) by
+   (not) Z.eqb instead. *)
+Lemma Zneq_bool_false_iff: forall x y : Z, x = y <-> Zneq_bool x y = false.
+Proof.
+  !intros;split;!intros.
+  -  subst.
+     unfold Zneq_bool.
+     rewrite Z.compare_refl;auto.
+  - unfold Zneq_bool in *.
+    destruct (x ?= y) eqn:h; try discriminate.
+    apply Z.compare_eq_iff.
+    assumption.
+Qed.
+
+
+Lemma Zeq_is_neq_bool : forall x y : Z, x <> y <-> Zeq_bool x y = false.
+Proof.
+  !intros.
+  split;!intro.
+  - destruct (Zeq_bool x y) eqn:h.
+    + apply Zeq_bool_eq in h.
+      contradiction.
+    + reflexivity.
+  - apply Zeq_bool_neq.
+    assumption.
+Qed.
+
+
+Lemma Zneq_bool_false :  forall x y : Z, x = y -> Zneq_bool x y = false.
+Proof.
+  intros x y H.
+  apply Zneq_bool_false_iff;easy.
+Qed.
+
+  
+Lemma Zneq_bool_true_iff: forall x y : Z, x <> y <-> Zneq_bool x y = true.
+Proof.
+  !intros;split;!intros.
+  - red in hneq.
+    rewrite <- Z.compare_eq_iff in hneq.
+    unfold Zneq_bool.
+    destruct (x ?= y); auto.
+  - unfold Zneq_bool in *.
+    destruct (x ?= y) eqn:h; try discriminate.
+    + rewrite  -> Z.compare_lt_iff in h.
+      apply Z.lt_neq;auto.
+    + rewrite -> Z.compare_gt_iff in h.
+      symmetry.
+      apply Z.lt_neq;auto.
+Qed.
+
+Lemma Zneq_bool_true :  forall x y : Z, x <> y -> Zneq_bool x y = true.
+Proof.
+  intros x y H.
+  apply Zneq_bool_true_iff;easy.
+Qed.
+
+Lemma Zeq_bool_Zneq_bool : forall x y, Zeq_bool x y = negb (Zneq_bool x y).
+Proof.
+  !intros x y.
+  !destruct (Z.eq_decidable x y).
+  - generalize heq_x.
+    !intro .
+    apply Zneq_bool_false_iff in heq_x.
+    apply Zeq_is_eq_bool in heq_x1.
+    rewrite heq_x, heq_x1.
+    reflexivity.
+  - generalize hneq.
+    !intro .
+    apply Zneq_bool_true in hneq.
+    apply Zeq_is_neq_bool in hneq1.
+    rewrite hneq, hneq1.
+    reflexivity.
+Qed.
